refined axiom for ECC + factorizations
git-svn-id: svn+ssh://scm.gforge.inria.fr/svn/coqcert/trunk/cic-model@211 7b0040dd-6dd6-45fd-888d-7922243e4794

ModelECCW.v
@@ -5,71 +5,12 @@
 Require Import List Bool Models.
 Require Import ZF ZFsum ZFnats ZFrelations ZFord ZFfix ZFgrothendieck.
 Require Import ZFfunext ZFind_w.
-Require Import ModelZF.
+Require Import ModelZF ModelECC.
 
 Import BuildModel.
 Import T J R.
 
-(** Derived rules of the basic judgements *)
-
-Lemma typ_var0 : forall e n T,
-  match T, nth_error e n with
-    Some _, value T' => T' <> kind /\ sub_typ e (lift (S n) T') T
-  | _,_ => False end ->
-  typ e (Ref n) T.
-intros.
-case_eq T; intros.
- rewrite H0 in H.
- case_eq (nth_error e n); intros.
-  rewrite H1 in H.
-  destruct H.
-  apply typ_subsumption with (lift (S n) t); auto.
-   apply typ_var; trivial.
-
-   destruct t as [(t,tm)|]; simpl; try discriminate.
-   elim H; trivial.
-
-  rewrite H1 in H; contradiction.
-
- rewrite H0 in H; contradiction.
-Qed.
-
-
-(** Subtyping *)
-
-(*
-Definition sub_typ_covariant : forall e U1 U2 V1 V2,
-  U1 <> kind ->
-  eq_typ e U1 U2 ->
-  sub_typ (U1::e) V1 V2 ->
-  sub_typ e (Prod U1 V1) (Prod U2 V2).
-intros.
-apply sub_typ_covariant; trivial.
-intros.
-unfold eqX, lam, app.
-unfold inX in H2.
-unfold prod, ZFuniv_real.prod in H2; rewrite El_def in H2.
-apply cc_eta_eq in H2; trivial.
-Qed.
-*)
-
-(** Universes *)
-(*
-Lemma cumul_Type : forall e n, sub_typ e (type n) (type (S n)).
-red; simpl; intros.
-red; intros.
-apply ecc_incl; trivial.
-Qed.
-
-Lemma cumul_Prop : forall e, sub_typ e prop (type 0).
-red; simpl; intros.
-red; intros.
-apply G_trans with props; trivial.
- apply (grot_succ_typ gr).
-
- apply (grot_succ_in gr).
-Qed.
-*)
+Require Import Model_variance.
 
 (** Ordinals *)
 
@@ -78,22 +19,6 @@ Definition Ordt (o:set) : term := cst o.
 Definition typ_ord_kind : forall e o, typ e (Ordt o) kind.
 red; simpl; trivial.
 Qed.
-
-(*Lemma El_int_ord o i :
-  zero ∈ o ->
-  El (int (Ordt o) i) == o.*)
-
-Definition OSucc : term -> term.
-(*begin show*)
-intros o; left; exists (fun i => osucc (int o i)).
-(*end show*)
-do 2 red; intros.
-rewrite H; reflexivity.
-Defined.
-
-(*Lemma El_int_osucc O' i :
-  El (int (OSucct O') i) == osucc (int O' i).
-*)
 
 Lemma tyord_inv : forall e i o o',
   isOrd o' ->
@@ -106,6 +31,40 @@ red in H0.
 split; auto.
 apply isOrd_inv with o'; trivial.
 apply H0; trivial.
+Qed.
+
+Definition OSucc : term -> term.
+(*begin show*)
+intros o; left; exists (fun i => osucc (int o i)).
+(*end show*)
+do 2 red; intros.
+rewrite H; reflexivity.
+Defined.
+
+  Lemma var_mono_OSucc : forall e O,
+    var_mono e O ->
+    var_mono e (OSucc O).
+unfold var_mono; red; simpl; intros.
+unfold osucc in H1|-*.
+rewrite subset_ax in H1 |-*.
+destruct H1; split; auto.
+revert H1; apply power_mono.
+red; intros; eauto.
+revert H1; apply H; trivial.
+Qed.
+
+  Lemma typ_mono_OSucc : forall e O o,
+    isOrd o ->
+    typ_mono e O (Ordt o)->
+    typ_mono e (OSucc O) (Ordt (osucc o)).
+destruct 2.
+split.
+ apply var_mono_OSucc; trivial.
+
+ red; simpl; intros.
+ red.
+ destruct tyord_inv with (2:=H1)(3:=H2) as (_,?); trivial.
+ apply lt_osucc_compat; trivial.
 Qed.
 
 (** W *)
@@ -159,10 +118,6 @@ apply TI_morph_gen.
  rewrite H; reflexivity.
 Defined.
 
-(*Lemma El_int_W O i :
-  El (int (WI O) i) == cc_bot (TI (WF' i) (int O i)).
-*)
-
 Lemma typ_WI : forall eps O,
   isOrd eps ->
   typ e O (Ordt eps) ->
@@ -180,26 +135,6 @@ left; exists (fun i => couple (int x i) (int f i)).
 (* end show *)
 do 2 red; intros; apply couple_morph; apply int_morph; auto with *.
 Defined.
-
-
-Lemma in_int_not_kind T i x :
-  el T i x ->
-  T <> kind ->
-  x ∈ int T i.
-destruct T as [(?,?)|]; simpl; intros; trivial.
-elim H0; trivial.
-Qed.
-
-Lemma El_int_arr T U i :
-  int (Prod T (lift 1 U)) i == cc_arr (int T i) (int U i).
-simpl.
-apply cc_prod_ext.
- reflexivity.
-
- red; intros.
- rewrite simpl_int_lift.
- rewrite lift0_term; reflexivity.
-Qed.
 
 Lemma typ_Wc : forall O X F,
   typ e O (Ordt o) ->
@@ -233,7 +168,6 @@ Qed.
 
 
 (* Case analysis *)
-
 
 Definition W_CASE b w :=
   sigma_case (fun x f => cc_app (cc_app b x) f) w.
@@ -339,297 +273,15 @@ Qed.
 
 End Wtypes_typing.
 
-(********************************************************************************)
-(** Occurrences *)
-
-
-  (* Non-occurrence : interp do not depend on variables in set [f] *)
-  Definition noccur (f:nat->bool) (T:term) : Prop :=
-    forall i i',
-    (forall n, if f n then True else i n == i' n) ->
-    int T i == int T i'.
-
-  Lemma noc_var : forall f n, f n = false -> noccur f (Ref n).
-red; simpl; intros.
-specialize (H0 n).
-rewrite H in H0; trivial.
-Qed.
-
-  Lemma noc_kind : forall f, noccur f kind.
-red; simpl; reflexivity.
-Qed.
-
-  Lemma noc_prop : forall f, noccur f prop.
-red; simpl; reflexivity.
-Qed.
-
-  Lemma noc_app : forall f a b,
-    noccur f a -> noccur f b -> noccur f (App a b).
-unfold noccur; simpl; intros.
-rewrite (H _ _ H1).
-rewrite (H0 _ _ H1).
-reflexivity.
-Qed.
-
-
-(********************************************************************************)
-(** Judgements with variance *)
-
-Module Beq.
-Definition t := bool.
-Definition eq := @eq bool.
-Definition eq_equiv : Equivalence eq := eq_equivalence.
-Existing Instance eq_equiv.
-End Beq.
-Module B := VarMap.Make(Beq).
-
-Module OTeq.
-Definition t := option term.
-Definition eq := @eq (option term).
-Definition eq_equiv : Equivalence eq := eq_equivalence.
-Existing Instance eq_equiv.
-End OTeq.
-Module OT := VarMap.Make(OTeq).
-
-(* Environments with tags on ordinal and recursive function variables *)
-Record fenv := {
-  tenv : env;
-  ords : B.map; (* variables denoting ordinals *)
-  fixs : OT.map (* variables denoting recursive functions with their domain *)
-}.
-
-Definition tinj e :=
-  Build_fenv e (B.nil false) (OT.nil None).
-
-Definition push_var e T :=
-  Build_fenv (T::tenv e) (B.cons false (ords e)) (OT.cons None (fixs e)).
-
-Definition push_fun e dom rng :=
-  Build_fenv (Prod dom rng::tenv e)
-    (B.cons false (ords e)) (OT.cons (Some dom) (fixs e)).
-
-Definition push_ord e T :=
-  Build_fenv (T::tenv e) (B.cons true (ords e)) (OT.cons None (fixs e)).
-
-
-(* Additional judgments for fix body *)
-Definition val_mono (e:fenv) i i' :=
-    val_ok (tenv e) i /\
-    val_ok (tenv e) i' /\
-    forall n,
-    if ords e n then i n ⊆ i' n
-    else match fixs e n with
-      Some T => forall x, x ∈ int T (V.shift (S n) i) -> cc_app (i n) x == cc_app (i' n) x
-    | _ => i n == i' n
-    end.
-
-Lemma val_mono_refl : forall e i,
-  val_ok (tenv e) i -> val_mono e i i.
-split;[idtac|split]; simpl; auto with *.
-intro n.
-destruct (ords e n); auto with *.
-destruct (fixs e n); auto with *.
-Qed.
-
-Lemma val_push_var : forall e i i' x x' T,
-  val_mono e i i' ->
-  x == x' ->
-  x ∈ int T i ->
-  x' ∈ int T i' ->
-  T <> kind ->
-  val_mono (push_var e T) (V.cons x i) (V.cons x' i').
-destruct 1 as (?&?&?); split;[idtac|split]; trivial.
- unfold push_var; simpl.
- apply vcons_add_var; trivial.
-
- unfold push_var; simpl.
- apply vcons_add_var; trivial.
-
- destruct n as [|n]; simpl; auto.
- generalize (H1 n).
- destruct (ords e n); trivial.
-Qed.
-
-Lemma val_push_ord : forall e i i' x x' T,
-  val_mono e i i' ->
-  x ⊆ x' ->
-  x ∈ int T i ->
-  x' ∈ int T i' ->
-  T <> kind ->
-  val_mono (push_ord e T) (V.cons x i) (V.cons x' i').
-destruct 1 as (?&?&?); split;[idtac|split]; trivial.
- unfold push_ord; simpl.
- apply vcons_add_var; trivial.
-
- unfold push_ord; simpl.
- apply vcons_add_var; trivial.
-
- destruct n as [|n]; simpl; auto.
- generalize (H1 n).
- destruct (ords e n); trivial.
-Qed.
-
-
-Lemma val_push_fun : forall e i i' f g T U,
-  val_mono e i i' ->
-  f ∈ int (Prod T U) i ->
-  g ∈ int (Prod T U) i' ->
-  fcompat (int T i) f g ->
-  val_mono (push_fun e T U) (V.cons f i) (V.cons g i').
-destruct 1 as (?&?&?); split;[idtac|split]; trivial.
- unfold push_fun; simpl.
- apply vcons_add_var; trivial.
-
- unfold push_fun; simpl.
- apply vcons_add_var; trivial.
-
- destruct n as [|n]; simpl; auto.
- generalize (H1 n).
- destruct (ords e n); trivial.
-Qed.
-
-(** Function Extension judgment *)
-Definition fx_extends e dom M :=
-  forall i i', val_mono e i i' ->
-  fcompat (int dom i) (int M i) (int M i').
-
-(** Covariance judgment *)
-Definition fx_sub e M :=
-  forall i i', val_mono e i i' ->
-  forall x, x ∈ int M i -> x ∈ int M i'.
-
-(** Invariance *)
-Definition fx_equals e M :=
-  forall i i', val_mono e i i' -> int M i == int M i'.
-
-
-Lemma El_sub e T i i':
-  fx_sub e T ->
-  val_mono e i i' ->
-  int T i ⊆ int T i'.
-intros.
-apply H in H0.
-red; auto.
-Qed.
-Lemma El_eq e T i i':
-  fx_equals e T ->
-  val_mono e i i' ->
-  int T i == int T i'.
-intros.
-apply H in H0.
-rewrite H0; reflexivity.
-Qed.
-
-
-Definition spec_var e n :=
-  ords e n || match fixs e n with Some _ => true | _ => false end.
-
-  Lemma fx_eq_noc : forall e t,
-    noccur (spec_var e) t ->
-    fx_equals e t.
-unfold noccur, fx_equals, spec_var; intros.
-apply H; intros.
-destruct H0 as (_,(_,H0)).
-generalize (H0 n).
-destruct (ords e n); simpl; trivial.
-destruct (fixs e n); simpl; trivial.
-Qed.
-
-  Lemma fx_eq_app : forall e u v,
-    fx_equals e u ->
-    fx_equals e v ->
-    fx_equals e (App u v).
-unfold fx_equals; intros.
-specialize H with (1:=H1).
-specialize H0 with (1:=H1).
-simpl.
-rewrite H; rewrite H0; reflexivity.
-Qed.
-
-  Lemma fx_eq_abs : forall e T M,
-    T <> kind ->
-    fx_equals e T ->
-    fx_equals (push_var e T) M ->
-    fx_equals e (Abs T M).
-unfold fx_equals; intros.
-simpl.
-apply cc_lam_ext; eauto.
-red; intros.
-apply H1.
-specialize H0 with (1:=H2).
-apply val_push_var; auto.
-rewrite <- H4; rewrite <- H0; trivial.
-Qed.
-
-  Lemma fx_eq_rec_call : forall e n x T U,
-    ords e n = false ->
-    fixs e n = Some T ->
-    T <> kind ->
-    typ (tenv e) (Ref n) (Prod (lift (S n) T) U) ->
-    fx_equals e x ->
-    typ (tenv e) x (lift (S n) T) ->
-    fx_equals e (App (Ref n) x).
-unfold fx_equals; intros.
-simpl.
-specialize H3 with (1:=H5).
-rewrite <- H3.
-destruct H5 as (Hty,(Hty',Hrec)).
-specialize Hrec with n.
-rewrite H in Hrec; rewrite H0 in Hrec.
-apply Hrec.
-red in H4; specialize H4 with (1:=Hty); trivial.
-apply in_int_not_kind in H4; trivial.
-2:destruct T as [(T,Tm)|];simpl;[discriminate|elim H1;reflexivity].
-unfold lift in H4; rewrite int_lift_rec_eq in H4.
-rewrite V.lams0 in H4; trivial.
-Qed.
-
-  (* Covariance *)
-
-  Lemma fx_equals_sub : forall e M, fx_equals e M -> fx_sub e M.
-unfold fx_sub, fx_equals; intros.
-apply H in H0.
-rewrite <- H0; trivial.
-Qed.
-
-  Lemma var_sub : forall e n,
-    ords e n = true ->
-    fx_sub e (Ref n).
-unfold fx_sub; intros.
-destruct H0 as (_,(_,H0)).
-generalize (H0 n); rewrite H.
-simpl; intros.
-apply H2; trivial.
-Qed.
-
-Lemma fx_sub_prod : forall e T U,
-  T <> kind ->
-  fx_equals e T ->
-  fx_sub (push_var e T) U ->
-  fx_sub e (Prod T U).
-red; intros.
-red in H0; specialize H0 with (1:=H2).
-revert H3; simpl; apply cc_prod_covariant; intros.
- do 2 red; intros.
- rewrite H4; reflexivity.
-
- rewrite H0; reflexivity.
-
- apply El_sub with (1:=H1).
- apply val_push_var; auto with *.
- rewrite <- H0; trivial.
-Qed.
-
-
-  Lemma Wi_sub : forall e o A B O,
+  Lemma var_mono_Wi : forall e o A B O,
     isOrd o ->
     A <> kind ->
     typ (tenv e) O (Ordt o) ->
-    fx_equals e A ->
-    fx_equals (push_var e A) B ->
-    fx_sub e O ->
-    fx_sub e (WI A B O).
-unfold fx_sub, fx_sub.
+    var_equals e A ->
+    var_equals (push_var e A) B ->
+    var_mono e O ->
+    var_mono e (WI A B O).
+unfold var_mono.
 intros e o A B O oo Ank tyO eqA eqB subO i i' val_m x xty.
 destruct tyord_inv with (2:=tyO) (3:=proj1 val_m); trivial.
 destruct tyord_inv with (2:=tyO) (3:=proj1 (proj2 val_m)); trivial.
@@ -653,41 +305,15 @@ assert (x ∈ TI (WF' A B i') (int O i)).
  apply Bw_morph; reflexivity.
 Qed.
 
-  Lemma OSucc_sub : forall e O,
-    fx_sub e O ->
-    fx_sub e (OSucc O).
-unfold fx_sub; simpl; intros.
-unfold osucc in H1|-*.
-rewrite subset_ax in H1 |-*.
-destruct H1; split; auto.
-revert H1; apply power_mono.
-red; intros; eauto.
-Qed.
-
-  (* Function subtyping *)
-
-  Lemma fx_abs : forall e U T M,
-    T <> kind ->
-    fx_sub e T ->
-    fx_equals (push_var e T) M ->
-    typ (T::tenv e) M U ->
-    U <> kind ->
-    fx_extends e T (Abs T M).
-unfold fx_equals, fx_extends; intros.
-specialize El_sub with (1:=H0)(2:=H4); clear H0; intro H0.
-simpl.
-red; intros.
-rewrite cc_beta_eq; try assumption.
- assert (H5' := H0 _ H5).
- rewrite cc_beta_eq; trivial.
-  apply H1.
-  apply val_push_var; auto with *.
-
-  red; red; intros.
-  rewrite H7; reflexivity.
-
- red; red; intros.
- rewrite H7; reflexivity.
+  Lemma var_mono_Wi' : forall e o A B O,
+    isOrd o ->
+    A <> kind ->
+    typ_equals e A kind ->
+    typ_equals (push_var e A) B kind ->
+    typ_mono e O (Ordt o) ->
+    var_mono e (WI A B O).
+intros e o A B O oo Ank (eqA,_) (eqB,_) (subO,tyO).
+apply var_mono_Wi with (o:=o); trivial.
 Qed.
 
 (*****************************************************************************)
@@ -725,8 +351,8 @@ Section WFixRules.
   Let e := tenv E.
   Variable A B O U M : term.
   Hypothesis A_nk : A <> kind.
-  Hypothesis Aeq : fx_equals E A.
-  Hypothesis Beq : fx_equals (push_var E A) B.
+  Hypothesis Aeq : var_equals E A.
+  Hypothesis Beq : var_equals (push_var E A) B.
 
   Definition WIL n := WI (lift n A) (lift_rec n 1 B).
 
@@ -735,7 +361,7 @@ Section WFixRules.
     M (Prod (WIL 2 (OSucc (Ref 1)))
          (lift_rec 1 1 (subst_rec (OSucc (Ref 0)) 1 (lift_rec 1 2 U)))).
 
-  Hypothesis stab : fx_extends
+  Hypothesis stab : var_ext
     (push_fun (push_ord E (OSucc O)) (WIL 1 (Ref 0)) U)
     (WIL 2 (OSucc (Ref 1)))
     M.
@@ -768,8 +394,8 @@ Qed.
   Hint Resolve U'morph morph_fix_body ext_fun_ty.
 
 
-  Hypothesis fx_sub_U :
-    fx_sub (push_var (push_ord E (OSucc O)) (WIL 1 (OSucc (Ref 0)))) U.
+  Hypothesis var_mono_U :
+    var_mono (push_var (push_ord E (OSucc O)) (WIL 1 (OSucc (Ref 0)))) U.
 
 
 Lemma El_int_W_lift O' n i :
@@ -807,7 +433,6 @@ Qed.
 intros is_val Oo Oo' oo' yo y'o yO y'O yy' fty gty eqfg.
 apply val_push_fun.
  apply val_push_ord; auto.
- 3:discriminate.
   apply ole_lts; trivial.
 
   apply ole_lts; trivial.
@@ -840,9 +465,7 @@ Qed.
 Proof.
 intros.
 apply val_push_var; auto with *.
- 4:discriminate.
  apply val_push_ord; auto with *.
-  4:discriminate.
   apply val_mono_refl; trivial.
 
   apply ole_lts; auto.
@@ -871,15 +494,14 @@ Qed.
    U' i o x ⊆ U' i o' x'.
 Proof.
 intros.
-red in fx_sub_U.
+red in var_mono_U.
 assert (val_mono (push_var (push_ord E (OSucc O)) (WIL 1(OSucc(Ref 0))))
   (V.cons x (V.cons o i)) (V.cons x' (V.cons o' i))).
  apply val_mono_2; trivial.
  apply ty_O in H.
  apply in_int_not_kind in H;[|discriminate].
  apply isOrd_inv with infty; auto.
-red; intros.
-apply fx_sub_U with (x:=z) in H6; trivial.
+apply var_mono_U in H6; trivial.
 Qed.
 
   Lemma ty_fix_body : forall i o f,
@@ -1121,8 +743,8 @@ Qed.
 
 
 Lemma wfix_extend :
-  fx_sub E O ->
-  fx_extends E (WI A B O) (WFix O M).
+  var_mono E O ->
+  var_ext E (WI A B O) (WFix O M).
 intro subO.
 do 2 red; intros.
 assert (isval := proj1 H).
@@ -1178,11 +800,11 @@ Qed.
 
 
 Lemma wfix_equals :
-  fx_equals E O ->
-  fx_equals E (WFix O M).
+  var_equals E O ->
+  var_equals E (WFix O M).
 red; intros.
-assert (fxs: fx_sub E O).
- apply fx_equals_sub; trivial.
+assert (fxs: var_mono E O).
+ apply var_eq_sub; trivial.
 apply wfix_extend in fxs.
 red in fxs.
 specialize fxs with (1:=H0).
@@ -1226,9 +848,9 @@ Lemma typ_wfix' : forall infty e A B O U M T,
        typ (Prod (WIL A B 1 (Ref 0)) U :: OSucc O :: e) M
          (Prod (WIL A B 2 (OSucc (Ref 1)))
          (lift_rec 1 1 (subst_rec (OSucc (Ref 0)) 1 (lift_rec 1 2 U)))) ->
-       fx_extends (push_fun (push_ord (tinj e) (OSucc O)) (WIL A B 1 (Ref 0)) U)
+       var_ext (push_fun (push_ord (tinj e) (OSucc O)) (WIL A B 1 (Ref 0)) U)
          (WIL A B 2 (OSucc (Ref 1))) M ->
-       fx_sub (push_var (push_ord (tinj e) (OSucc O)) (WIL A B 1 (OSucc (Ref 0)))) U ->
+       var_mono (push_var (push_ord (tinj e) (OSucc O)) (WIL A B 1 (OSucc (Ref 0)))) U ->
        sub_typ e (Prod (WI A B O) (subst_rec O 1 U)) T ->
        typ e (WFix O M) T.
 intros.
@@ -1237,177 +859,6 @@ apply typ_subsumption with (Prod (WI A B O) (subst_rec O 1 U)); auto.
 change e with (tenv (tinj e)).
 apply typ_wfix with (infty:=infty); trivial.
 Qed.
-
-(****************************************************************************************)
-(** Compound judgements : typing + variance *)
-
-Definition typ_ext e M A B :=
-  fx_extends e A M /\ typ (tenv e) M (Prod A B).
-
-Definition typ_mono e M T :=
-  fx_sub e M /\ typ (tenv e) M T.
-
-Definition typ_impl e M T :=
-  fx_equals e M /\ typ (tenv e) M T.
-
-Instance typ_impl_morph e : Proper (eq_term ==> eq_term ==> iff) (typ_impl e).
-apply morph_impl_iff2; auto with *.
-do 4 red; intros.
-destruct H1; split.
- red; intros.
- rewrite <- H; eauto.
-
- rewrite <- H; rewrite <- H0; eauto.
-Qed.
-
-Lemma typ_var_impl : forall e n t T,
-    spec_var e n = false ->
-    nth_error (tenv e) n = value t ->
-    t <> kind ->
-    T <> kind ->
-    sub_typ (tenv e) (lift (S n) t) T ->
-    typ_impl e (Ref n) T.
-intros.
-split.
- apply fx_eq_noc; apply noc_var; trivial.
-
- apply typ_subsumption with (lift (S n) t); trivial.
-  apply typ_var; trivial.
-
-  destruct t as [(t,tm)|]; simpl in *; auto.
-  discriminate.
-Qed.
-
-  Lemma impl_abs : forall e s1 U T T' M,
-    T <> kind ->
-    U <> kind ->
-    s1=prop \/ s1=kind ->
-    eq_typ (tenv e) T T' ->
-    typ_impl e T s1 ->
-    typ_impl (push_var e T) M U ->
-    typ_impl e (Abs T M) (Prod T' U).
-intros.
-destruct H3; destruct H4.
-split.
- apply fx_eq_abs; trivial.
-
- apply typ_conv with (Prod T U); auto.
-  apply typ_abs; trivial.
-
-  apply eq_typ_prod; trivial.
-  reflexivity.
-
- discriminate.
-Qed.
-
-Lemma impl_app : forall e u v V Ur T,
-  T <> kind ->
-  V <> kind ->
-  Ur <> kind ->
-  sub_typ (tenv e) (subst v Ur) T ->
-  typ_impl e u (Prod V Ur) ->
-  typ_impl e v V ->
-  typ_impl e (App u v) T.
-intros.
-destruct H3.
-destruct H4.
-split.
- apply fx_eq_app; trivial.
-
- apply typ_subsumption with (subst v Ur); trivial.
-  apply typ_app with V; auto.
-
-  destruct Ur as [(Ur,Urm)|]; simpl; trivial.
-  discriminate.
-Qed.
-
-  Lemma Wi_fx_sub : forall e o A B O,
-    isOrd o ->
-    A <> kind ->
-    typ_impl e A kind ->
-    typ_impl (push_var e A) B kind ->
-    typ_mono e O (Ordt o) ->
-    fx_sub e (WI A B O).
-intros e o A B O oo Ank (eqA,_) (eqB,_) (subO,tyO).
-apply Wi_sub with (o:=o); trivial.
-Qed.
-
-  Lemma OSucc_fx_sub : forall e O o,
-    isOrd o ->
-    typ_mono e O (Ordt o)->
-    typ_mono e (OSucc O) (Ordt (osucc o)).
-destruct 2.
-split.
- apply OSucc_sub; trivial.
-
- red; simpl; intros.
- red.
- destruct tyord_inv with (2:=H1)(3:=H2) as (_,?); trivial.
- apply lt_osucc_compat; trivial.
-Qed.
-
-  Lemma typ_var_mono : forall e n t T,
-    ords e n = true ->
-    nth_error (tenv e) n = value t ->
-    T <> kind ->
-    t <> kind ->
-    sub_typ (tenv e) (lift (S n) t) T ->
-    typ_mono e (Ref n) T.
-intros.
-split.
- apply var_sub; trivial.
-
- apply typ_subsumption with (lift (S n) t); trivial.
-  apply typ_var; trivial.
-
-  destruct t as [(t,tm)|]; simpl in *; auto.
-  discriminate.
-Qed.
-
-  Lemma ext_abs : forall e U T M,
-    T <> kind ->
-    U <> kind ->
-    typ_mono e T kind ->
-    typ_impl (push_var e T) M U ->
-    typ_ext e (Abs T M) T U.
-intros.
-destruct H1; destruct H2; split.
- apply fx_abs with U; trivial.
-
- apply typ_abs; trivial.
-Qed.
-
-(*************)
-
-  Lemma impl_call : forall e n x t u T,
-    ords e n = false ->
-    fixs e n = Some t ->
-    T <> kind ->
-    t <> kind ->
-    u <> kind ->
-    nth_error (tenv e) n = value (Prod t u) ->
-    sub_typ (tenv e) (subst x (lift_rec (S n) 1 u)) T ->
-    typ_impl e x (lift (S n) t) ->
-    typ_impl e (App (Ref n) x) T.
-intros.
-destruct H6.
-assert (typ (tenv e) (Ref n) (Prod (lift (S n) t) (lift_rec (S n) 1 u))).
- apply typ_var0; rewrite H4; split;[discriminate|].
- apply sub_refl.
-
- unfold lift; rewrite eq_lift_prod.
- reflexivity.
-split.
- apply fx_eq_rec_call with t (lift_rec (S n) 1 u); trivial.
-
- apply typ_subsumption with (subst x (lift_rec (S n) 1 u)); auto.
- 2:destruct u as [(u,um)|]; trivial.
- 2:discriminate.
- apply typ_app with (lift (S n) t); trivial.
- destruct t as [(t,tm)|]; trivial.
- discriminate.
-Qed.
-
 
 Lemma typ_wfix'' : forall infty e A B O U M T,
        isOrd infty ->
@@ -1429,13 +880,13 @@ Qed.
   Lemma typ_ext_fix : forall eps e A B O U M,
     isOrd eps ->
     A <> kind ->
-    typ_impl e A kind ->
-    typ_impl (push_var e A) B kind ->
+    typ_equals e A kind ->
+    typ_equals (push_var e A) B kind ->
     typ_mono e O (Ordt eps) ->
     typ_ext (push_fun (push_ord e (OSucc O)) (WI (lift 1 A) (lift_rec 1 1 B) (Ref 0)) U) M
       (WI (lift 2 A) (lift_rec 2 1 B) (OSucc (Ref 1)))
       (lift_rec 1 1 (subst_rec (OSucc (Ref 0)) 1 (lift_rec 1 2 U))) ->
-    fx_sub (push_var (push_ord e (OSucc O)) (WI (lift 1 A) (lift_rec 1 1 B) (OSucc (Ref 0)))) U ->
+    var_mono (push_var (push_ord e (OSucc O)) (WI (lift 1 A) (lift_rec 1 1 B) (OSucc (Ref 0)))) U ->
     typ_ext e (WFix O M) (WI A B O) (subst_rec O 1 U).
 intros eps e A B O U M eps_ord Ank tyA tyB tyO tyM tyU.
 destruct tyO as (inclO,tyO).
@@ -1448,87 +899,23 @@ destruct tyA as (eqA,tyA).
 apply wfix_extend with eps U; trivial.
 Qed.
 
-  Lemma typ_impl_fix : forall eps e A B O U M,
+  Lemma typ_equals_fix : forall eps e A B O U M,
     isOrd eps ->
     A <> kind ->
-    typ_impl e A kind ->
-    typ_impl (push_var e A) B kind ->
-    typ_impl e O (Ordt eps) ->
+    typ_equals e A kind ->
+    typ_equals (push_var e A) B kind ->
+    typ_equals e O (Ordt eps) ->
     typ_ext (push_fun (push_ord e (OSucc O)) (WI (lift 1 A) (lift_rec 1 1 B) (Ref 0)) U) M
       (WI (lift 2 A) (lift_rec 2 1 B) (OSucc (Ref 1)))
       (lift_rec 1 1 (subst_rec (OSucc (Ref 0)) 1 (lift_rec 1 2 U))) ->
-    fx_sub (push_var (push_ord e (OSucc O)) (WI (lift 1 A) (lift_rec 1 1 B) (OSucc (Ref 0)))) U ->
-    typ_impl e (WFix O M) (Prod (WI A B O) (subst_rec O 1 U)).
+    var_mono (push_var (push_ord e (OSucc O)) (WI (lift 1 A) (lift_rec 1 1 B) (OSucc (Ref 0)))) U ->
+    typ_equals e (WFix O M) (Prod (WI A B O) (subst_rec O 1 U)).
 intros eps e A B O U M eps_ord Ank (eqA,tyA) (eqB,_) (inclO,tyO) (extM,tyM) tyU.
 assert (tyF: typ (tenv e) (WFix O M) (Prod (WI A B O) (subst_rec O 1 U))).
  apply typ_wfix with eps; trivial.
 split; trivial.
 apply wfix_equals with eps A B U; trivial.
 Qed.
-
-(** Universes *)
-
-Require Import ZFecc.
-
-Definition type (n:nat) := cst (ecc (S n)).
-
-Lemma typ_Prop : forall e, typ e prop (type 0).
-red; intros; simpl.
-apply G_trans with (grot_succ (ZFcoc.props)); auto.
- apply (grot_succ_typ gr).
-
- apply (grot_succ_in gr).
-
- apply (grot_succ_in gr).
-Qed.
-
-Lemma typ_Type : forall e n, typ e (type n) (type (S n)).
-red; intros; simpl.
-apply (grot_succ_in gr).
-Qed.
-
-Lemma cumul_Type : forall e n, sub_typ e (type n) (type (S n)).
-red; simpl; intros.
-red; intros.
-apply ecc_incl with (n:=S n); trivial.
-Qed.
-
-Lemma cumul_Prop : forall e, sub_typ e prop (type 0).
-red; simpl; intros.
-red; intros.
-apply G_trans with ZFcoc.props; trivial.
- apply (grot_succ_typ gr).
-apply G_trans with (grot_succ ZFcoc.props); trivial.
- apply (grot_succ_typ gr).
-
- apply (grot_succ_in gr).
-
- apply (grot_succ_in gr).
-Qed.
-
-Lemma typ_prod2 : forall e n T U,
-  typ e T (type n) ->
-  typ (T :: e) U (type n) ->
-  typ e (Prod T U) (type n).
-Proof.
-red; intros e n T U ty_T ty_U i is_val.
-apply G_cc_prod.
- apply ecc_grot.
-
- red; red; intros.
- rewrite H0; auto with *.
-
- apply ty_T; trivial.
-
- intros.
- red in ty_U.
- change (int (type n) i) with (int (type n) (V.cons x i)).
- apply in_int_not_kind.
- 2:discriminate.
- apply ty_U.
- apply vcons_add_var; auto.
-Qed.
-
 
 (** * W-types and universes. *)
 
@@ -1546,7 +933,7 @@ clear tyO.
 red in tyA; specialize tyA with (1:=is_val).
 apply in_int_not_kind in tyA.
 2:discriminate.
-assert (G_B : forall a, a ∈ int A i -> int B (V.cons a i) ∈ ecc (S n)).
+assert (G_B : forall a, a ∈ int A i -> int B (V.cons a i) ∈ ZFecc.ecc (S n)).
  intros.
  assert (val_ok (A::e) (V.cons a i)).
   apply vcons_add_var; trivial.
@@ -1555,10 +942,10 @@ assert (G_B : forall a, a ∈ int A i -> int B (V.cons a i) ∈ ecc (S n)).
  2:discriminate.
  trivial.
 apply G_incl with (TI (WF' A B i) (W_ord (int A i) (fun x => int B (V.cons x i)))); trivial.
- apply (grot_succ_typ gr).
+ apply (ZFecc.ecc_grot (S n)).
 
  apply G_TI; trivial.
-  apply (grot_succ_typ gr).
+  apply (ZFecc.ecc_grot (S n)).
 
   apply WF'_morph; auto with *.
 
@@ -1574,206 +961,16 @@ apply G_incl with (TI (WF' A B i) (W_ord (int A i) (fun x => int B (V.cons x i))
   apply G_W_ord; auto.
    apply Bw_morph; reflexivity.
 
-   apply (grot_succ_typ gr).
+   apply (ZFecc.ecc_grot (S n)).
 
-   change (omega ∈ ecc (S n)); auto.
+   change (omega ∈ ZFecc.ecc (S n)); auto.
 
   intros.
   apply G_W_F; auto.
    apply Bw_morph; reflexivity.
 
-   apply (grot_succ_typ gr).
+   apply (ZFecc.ecc_grot (S n)).
 
  apply W_stages; trivial.
  apply Bw_morph; reflexivity.
 Qed.
-
-
-(*
-(************************************************************************)
-(** One example of derived principles:
-    - the standard recursor for W
-*)
-Section Example.
-
-Definition nat_ind_typ :=
-   Prod (Prod (NatI (Ord omega)) prop) (* P : nat -> Prop *)
-  (Prod (App (Ref 0) Zero)
-  (Prod (Prod (NatI (Ord omega)) (Prod (App (Ref 2) (Ref 0))
-                        (App (Ref 3) (App (Succ (Ord omega)) (Ref 1)))))
-  (Prod (NatI (Ord omega)) (App (Ref 3) (Ref 0))))).
-
-Definition nat_ind :=
-   Abs (*P*)(Prod (NatI (Ord omega)) prop) (* P : nat -> Prop *)
-  (Abs (*fZ*) (App (Ref 0) Zero)
-  (Abs (*fS*) (Prod (*n*)(NatI (Ord omega)) (Prod (App (Ref 2) (Ref 0))
-                                   (App (Ref 3) (App (Succ (Ord omega)) (Ref 1)))))
-  (NatFix (Ord omega)
-    (*o,Hrec*)
-    (Abs (*n*)(NatI (OSucc (Ref 1)))
-      (Natcase
-        (Ref 4)
-        (*k*)(App (App (Ref 4) (Ref 0))
-                  (App (Ref 2) (Ref 0)))
-        (Ref 0)))))).
-
-
-
-Lemma nat_ind_def :
-  forall e, typ e nat_ind nat_ind_typ.
-assert (eq_trm Nat (NatI (Ord omega))).
- red; simpl.
- red; unfold NAT; reflexivity.
-unfold nat_ind, nat_ind_typ; intros.
-apply typ_abs; try discriminate.
-apply typ_abs; try discriminate.
-apply typ_abs; try discriminate.
-
-set (E0 := Prod (NatI (Ord omega))
-                 (Prod (App (Ref 2) (Ref 0))
-                    (App (Ref 3) (App (SuccI (Ord omega)) (Ref 1))))
-               :: App (Ref 0) Zero :: Prod (NatI (Ord omega)) prop :: e) in |-*.
-change E0 with (tenv (tinj E0)).
-apply typ_nat_fix'' with (osucc omega) (App (Ref 4) (Ref 0)); auto.
- (* sub *)
- apply sub_refl.
- apply eq_typ_prod.
-  reflexivity.
-
-  eapply eq_typ_morph;[reflexivity| |reflexivity].
-  simpl; do 2 red; simpl; intros.
-  unfold V.lams, V.shift; simpl.
-  apply cc_app_morph; apply H0.
-
- (* ord *)
- red; simpl; intros.
- apply lt_osucc; trivial.
-
- (* codom mono *)
- split.
-  apply fx_equals_sub.
-  apply fx_eq_noc.
-  apply noc_app.
-   apply noc_var; reflexivity.
-   apply noc_var; reflexivity.
-
-  red; intros; simpl; exact I.
-
- (* fix body *)
- apply ext_abs; try discriminate.
-  apply Wi_fx_sub with (o:=osucc (osucc omega)); auto.
-  apply OSucc_fx_sub; auto.
-  apply typ_var_mono with (OSucct (Ord omega)); auto; try discriminate.
-  red; simpl; intros; trivial.
-
-  apply impl_natcase with (osucc omega) (Ref 2) (Ref 5); auto.
-   eapply typ_var_mono.
-    compute; reflexivity.
-    simpl; reflexivity.
-    discriminate.
-
-    simpl tenv; apply sub_refl.
-    red; simpl; intros; reflexivity.
-
-   simpl tenv.
-   apply sub_refl.
-   red; simpl; intros.
-   unfold V.lams, V.shift; simpl.
-   reflexivity.
-
-   (* branch 0 *)
-   eapply typ_var_impl.
-    compute; reflexivity.
-    simpl nth_error.
-    reflexivity.
-    discriminate.
-
-    apply sub_refl; red; simpl; intros.
-    unfold V.lams, V.shift; simpl.
-    reflexivity.
-
-   (* branch S *)
-   apply impl_app with (App (Ref 6) (Ref 0))
-     (App (Ref 7) (App (SuccI (Ref 4)) (Ref 1))); try discriminate.
-    simpl tenv.
-    apply sub_refl; red; intros; simpl.
-    unfold V.lams, V.shift; simpl.
-    reflexivity.
-
-    apply impl_app with (NatI (Ord omega))
-      (Prod (App (Ref 7) (Ref 0)) (App (Ref 8) (App (SuccI (Ord omega)) (Ref 1))));
-      try discriminate.
-     simpl tenv.
-     unfold subst; rewrite eq_subst_prod.
-     apply sub_typ_covariant.
-      red; simpl; intros; reflexivity.
-
-     apply sub_refl.
-     red; intros; simpl.
-     apply cc_app_morph; [reflexivity|].
-     assert (i 1 ∈ Wi (i 4)).
-      generalize (H0 1 _ (eq_refl _)); simpl.
-      unfold V.lams, V.shift; simpl.
-      trivial.
-     rewrite beta_eq.
-      rewrite beta_eq; auto with *.
-       reflexivity.
-       red; intros; apply inr_morph; trivial.
-
-      red; intros; apply inr_morph; trivial.
-
-      apply Wi_NAT in H1; trivial.
-      generalize (H0 4 _ (eq_refl _)); simpl; intro.
-      apply isOrd_inv with (osucc omega); auto.
-
-     eapply typ_var_impl.
-      compute; reflexivity.
-      simpl; reflexivity.
-      discriminate.
-
-      apply sub_refl.
-      red; intros; simpl.
-      unfold V.lams, V.shift; simpl.
-      reflexivity.
-
-     eapply typ_var_impl.
-      compute; reflexivity.
-      simpl; reflexivity.
-      discriminate.
-
-      red; intros; simpl.
-      simpl in H1.
-      unfold V.lams, V.shift in H1; simpl in H1.
-      apply Wi_NAT in H1; trivial.
-      generalize (H0 3 _ (eq_refl _)); simpl; intro.
-      apply isOrd_inv with (osucc omega); auto.
-
-    eapply impl_call.
-     compute; trivial.
-     simpl; reflexivity.
-     discriminate.
-     2:simpl; reflexivity.
-     discriminate.
-
-     apply sub_refl; red; intros; simpl.
-     unfold V.lams, V.shift; simpl.
-     reflexivity.
-
-     eapply typ_var_impl.
-      compute; reflexivity.
-      simpl; reflexivity.
-      discriminate.
-
-      apply sub_refl; red; intros; simpl.
-      reflexivity.
-
-   (* Scrutinee *)
-   eapply typ_var_impl.
-    compute; reflexivity.
-    simpl; reflexivity.
-    discriminate.
-
-    apply sub_refl; red; intros; simpl.
-    reflexivity.
-Qed.
-*)
