ModelNat_sized.v
@@ -7,106 +7,7 @@ Import ModelZF.CCM.
 Import ModelZF.BuildModel.
 Import T R J.
 
-(** Derived rules of the basic judgements *)
-
-Lemma eq_typ_betar : forall e N T M,
-  typ e N T ->
-  T <> kind ->
-  eq_typ e (App (Abs T M) N) (subst N M).
-intros.
-apply eq_typ_beta; trivial.
- reflexivity.
- reflexivity.
-Qed.
-
-Lemma typ_var0 : forall e n T,
-  match nth_error e n with
-    value T' => T' <> kind /\ sub_typ e (lift (S n) T') T
-  | _ => False end ->
-  typ e (Ref n) T.
-intros.
-case_eq (nth_error e n); intros.
- rewrite H0 in H.
- destruct H.
- apply typ_subsumption with (lift (S n) t); auto.
-  apply typ_var; trivial.
-
-  destruct t as [(t,tm)|]; simpl; try discriminate.
-  elim H; trivial.
-
- rewrite H0 in H; contradiction.
-Qed.
-
-Lemma typ_kind_univ e t : typ e t kind.
-red; simpl; auto.
-Qed.
-
-(** Subtyping *)
-
-Definition sub_typ_covariant : forall e U1 U2 V1 V2,
-  eq_typ e U1 U2 ->
-  sub_typ (U1::e) V1 V2 ->
-  sub_typ e (Prod U1 V1) (Prod U2 V2).
-unfold sub_typ; simpl; intros.
-apply cc_prod_covariant with (4:=H2).
- red; red; intros.
- rewrite H4; auto with *.
-
- apply H; trivial.
-
- red; intros.
- apply H0; trivial.
- apply vcons_add_var; trivial.
-Qed.
-
-(** Universes *)
-
-Definition type (n:nat) := cst (ecc n).
-
-Lemma typ_Prop : forall e, typ e prop (type 0).
-red; intros; simpl.
-apply (grot_succ_in gr).
-Qed.
-
-Lemma typ_Type : forall e n, typ e (type n) (type (S n)).
-red; intros; simpl.
-apply (grot_succ_in gr).
-Qed.
-
-Lemma cumul_Type : forall e n, sub_typ e (type n) (type (S n)).
-red; simpl; intros.
-red; intros.
-apply ecc_incl; trivial.
-Qed.
-
-Lemma cumul_Prop : forall e, sub_typ e prop (type 0).
-red; simpl; intros.
-red; intros.
-apply G_trans with props; trivial.
- apply (grot_succ_typ gr).
-
- apply (grot_succ_in gr).
-Qed.
-
-Lemma typ_prod2 : forall e n T U,
-  typ e T (type n) ->
-  typ (T :: e) U (type n) ->
-  typ e (Prod T U) (type n).
-Proof.
-unfold typ, Prod; simpl; red; intros e n T U ty_T ty_U i is_val.
-apply G_cc_prod.
- apply ecc_grot.
-
- red; red; intros.
- rewrite H0; auto with *.
-
- apply ty_T; trivial.
-
- intros.
- apply ty_U.
- apply vcons_add_var; auto.
-Qed.
-
+Require Import Model_variance.
 
 (** * Ordinals *)
 
@@ -218,11 +119,12 @@ apply NATi_morph.
 rewrite H; reflexivity.
 Defined.
 
-(** NB: type 0 is the universe of hereditarily finite sets,
-    so NAT is in type 1. *)
+Require ModelECC.
+Import ModelECC.WithoutFinitistUniverse.
+
 Lemma typ_natI_type : forall e O,
   typ_ord e O ->
-  typ e (NatI O) (type 1).
+  typ e (NatI O) (type 0).
 red; intros.
 apply H in H0.
 change (NATi (int O i) ∈ ecc 1).
@@ -404,275 +306,6 @@ apply typ_subsumption with (App P n); auto.
 apply typ_natcase with O; trivial.
 Qed.
 
-(********************************************************************************)
-(** * Variance *)
-
-(** Occurrences *)
-
-Module Beq.
-Definition t := bool.
-Definition eq := @eq bool.
-Definition eq_equiv : Equivalence eq := eq_equivalence.
-Existing Instance eq_equiv.
-End Beq.
-Module B := VarMap.Make(Beq).
-
-
-  (* Non-occurrence : interp do not depend on variables in set [f] *)
-  Definition noccur (f:B.map) (T:term) : Prop :=
-    forall i i',
-    (forall n, if f n then True else i n == i' n) ->
-    int T i == int T i'.
-
-  Lemma noc_var : forall f n, f n = false -> noccur f (Ref n).
-red; simpl; intros.
-specialize (H0 n).
-rewrite H in H0; trivial.
-Qed.
-
-  Lemma noc_kind : forall f, noccur f kind.
-red; simpl; reflexivity.
-Qed.
-
-  Lemma noc_prop : forall f, noccur f prop.
-red; simpl; reflexivity.
-Qed.
-
-  Lemma noc_app : forall f a b,
-    noccur f a -> noccur f b -> noccur f (App a b).
-unfold noccur; simpl; intros.
-rewrite (H _ _ H1).
-rewrite (H0 _ _ H1).
-reflexivity.
-Qed.
-
-Lemma noc_abs a b f :
-  noccur f a ->
-  noccur (B.cons false f) b ->
-  noccur f (Abs a b).
-red; simpl; intros.
-apply cc_lam_ext.
- apply H; trivial.
-
- red; intros.
- apply H0.
- destruct n; simpl; trivial.
- apply H1.
-Qed.
-
-Lemma noc_prod a b f :
-  noccur f a ->
-  noccur (B.cons false f) b ->
-  noccur f (Prod a b).
-red; simpl; intros.
-apply cc_prod_ext.
- apply H; trivial.
-
- red; intros.
- apply H0.
- destruct n; simpl; trivial.
- apply H1.
-Qed.
-
-Ltac noc_tac :=
-  lazymatch goal with 
-    |- noccur _ (App _ _) => apply noc_app; noc_tac
-  | |- noccur _ (Abs _ _) => apply noc_abs; noc_tac
-  | |- noccur _ (Prod _ _) => apply noc_prod; noc_tac
-  | |- noccur _ (Ref _) => apply noc_var; reflexivity
-  | |- noccur _ _ => try (red; reflexivity) (* closed case *)
-  end.
-
-
-(********************************************************************************)
-(** ** Judgements with variance *)
-
-
-(** Mark stage-irrelevant functions (domain information have to be repeated) *)
-Module OTeq.
-Definition t := option term.
-Definition eq := @eq (option term).
-Definition eq_equiv : Equivalence eq := eq_equivalence.
-Existing Instance eq_equiv.
-End OTeq.
-Module OT := VarMap.Make(OTeq).
-
-(** Environments with tags on ordinal and recursive function variables *)
-Record fenv := {
-  tenv : env;
-  ords : B.map; (* variables denoting ordinals *)
-  fixs : OT.map (* variables denoting recursive functions with their domain *)
-}.
-
-Definition tinj e :=
-  Build_fenv e (B.nil false) (OT.nil None).
-
-(** Pushing an ordinary variable *)
-Definition push_var e T :=
-  Build_fenv (T::tenv e) (B.cons false (ords e)) (OT.cons None (fixs e)).
-
-(** Pushing a stage-irrelevant function *)
-Definition push_fun e dom rng :=
-  Build_fenv (Prod dom rng::tenv e)
-    (B.cons false (ords e)) (OT.cons (Some dom) (fixs e)).
-
-(** Pushing an ordinal (stage) variable *)
-Definition push_ord e T :=
-  Build_fenv (T::tenv e) (B.cons true (ords e)) (OT.cons None (fixs e)).
-
-
-(** Semantics of contexts for variance judgments:
-    - ordinal variables follow the ordinal order
-    - stage-irrelevant function have to be compatible
-    - regular variables have to be the same
-*)
-
-Definition val_mono (e:fenv) i i' :=
-    val_ok (tenv e) i /\
-    val_ok (tenv e) i' /\
-    forall n,
-    if ords e n then i n ⊆ i' n
-    else match fixs e n with
-      Some T => fcompat (int T (V.shift (S n) i)) (i n) (i' n)
-    | _ => i n == i' n
-    end.
-
-Lemma val_mono_refl : forall e i,
-  val_ok (tenv e) i -> val_mono e i i.
-split;[idtac|split]; simpl; auto with *.
-intro n.
-destruct (ords e n); auto with *.
-destruct (fixs e n); auto with *.
-red; auto with *.
-Qed.
-
-Lemma val_push_var : forall e i i' x x' T,
-  val_mono e i i' ->
-  x == x' ->
-  el T i x ->
-  el T i' x' ->
-  val_mono (push_var e T) (V.cons x i) (V.cons x' i').
-destruct 1 as (?&?&?); split;[idtac|split]; trivial.
- unfold push_var; simpl.
- apply vcons_add_var0; trivial.
-
- unfold push_var; simpl.
- apply vcons_add_var0; trivial.
-
- destruct n as [|n]; simpl; auto.
- generalize (H1 n).
- destruct (ords e n); trivial.
-Qed.
-
-Lemma val_push_ord : forall e i i' x x' T,
-  val_mono e i i' ->
-  x ⊆ x' ->
-  el T i x ->
-  el T i' x' ->
-  val_mono (push_ord e T) (V.cons x i) (V.cons x' i').
-destruct 1 as (?&?&?); split;[idtac|split]; trivial.
- unfold push_ord; simpl.
- apply vcons_add_var0; trivial.
-
- unfold push_ord; simpl.
- apply vcons_add_var0; trivial.
-
- destruct n as [|n]; simpl; auto.
- generalize (H1 n).
- destruct (ords e n); trivial.
-Qed.
-
-Lemma val_push_fun : forall e i i' f g T U,
-  val_mono e i i' ->
-  f ∈ prod (int T i) (fun x => int U (V.cons x i)) ->
-  g ∈ prod (int T i') (fun x => int U (V.cons x i')) ->
-  fcompat (int T i) f g ->
-  val_mono (push_fun e T U) (V.cons f i) (V.cons g i').
-destruct 1 as (?&?&?); split;[idtac|split]; trivial.
- unfold push_fun; simpl.
- apply vcons_add_var0; trivial.
-
- unfold push_fun; simpl.
- apply vcons_add_var0; trivial.
-
- destruct n as [|n]; simpl; auto.
- generalize (H1 n).
- destruct (ords e n); trivial.
-Qed.
-
-(** Invariance judgement *)
-Definition var_equals e M :=
-  forall i i', val_mono e i i' -> int M i == int M i'.
-
-(** Function Extension judgment *)
-Definition var_compat e dom M :=
-  forall i i', val_mono e i i' ->
-  fcompat (int dom i) (int M i) (int M i').
-
-(** Covariance judgment *)
-Definition var_mono e M :=
-  forall i i', val_mono e i i' ->
-  int M i ⊆ int M i'.
-
-
-(** Invariance rules *)
-  Definition spec_var e n :=
-    ords e n || match fixs e n with Some _ => true | _ => false end.
-
-  Lemma var_eq_noc : forall e t,
-    noccur (spec_var e) t ->
-    var_equals e t.
-unfold noccur, var_equals, spec_var; intros.
-apply H; intros.
-destruct H0 as (_,(_,H0)).
-generalize (H0 n).
-destruct (ords e n); simpl; trivial.
-destruct (fixs e n); simpl; trivial.
-Qed.
-
-  Lemma var_eq_app : forall e u v,
-    var_equals e u ->
-    var_equals e v ->
-    var_equals e (App u v).
-unfold var_equals; intros.
-specialize H with (1:=H1).
-specialize H0 with (1:=H1).
-simpl.
-rewrite H; rewrite H0; reflexivity.
-Qed.
-
-  Lemma var_eq_abs : forall e T M,
-    var_equals e T ->
-    var_equals (push_var e T) M ->
-    var_equals e (Abs T M).
-unfold var_equals; intros.
-simpl.
-apply lam_ext; auto.
-red; intros.
-apply H0.
-specialize H with (1:=H1).
-apply val_push_var; auto.
- change (el T i' y2).
- apply in_int_el; trivial.
- rewrite <- H3; rewrite <- H; trivial.
-Qed.
-
-  Lemma var_eq_prod : forall e T U,
-    var_equals e T ->
-    var_equals (push_var e T) U ->
-    var_equals e (Prod T U).
-red; simpl; intros.
-specialize (H _ _ H1).
-apply cc_prod_ext; trivial.
-red; intros.
-apply H0.
-apply val_push_var; auto with *.
-change (el T i' x').
-rewrite <- H3.
-apply in_int_el.
-rewrite <- H; trivial.
-Qed.
-
   Lemma var_eq_NATi : forall e O,
     typ_ord (tenv e) O ->
     var_equals e O ->
@@ -709,67 +342,20 @@ assert (int c i ∈ NATi (osucc (int O i))).
  destruct H4 as (H4,_).
  apply tyc in H4; trivial.
 apply NATCASE_morph_gen; intros; auto.
- apply H3; trivial.
-
- apply H1; trivial.
-
- apply H2.
- red in H0; specialize H0 with (1:=H4).
- rewrite H5 in H.
- apply SUCCi_inv_typ in H; auto.
- apply val_push_var; simpl; auto.
- rewrite <- H6.
- clear H5 H6 x'; revert x H.
- apply TI_mono; auto.
+apply H2.
+red in H0; specialize H0 with (1:=H4).
+rewrite H5 in H.
+apply SUCCi_inv_typ in H; auto.
+apply val_push_var; simpl; auto.
+rewrite <- H6.
+clear H5 H6 x'; revert x H.
+apply TI_mono; auto.
 Qed.
 
-(** Stage-irrelevance rules *)
-  Lemma var_comp_ref : forall e dom n T,
-    ords e n = false ->
-    fixs e n = Some T ->
-    T <> kind ->
-    eq_typ (tenv e) (lift (S n) T) dom ->
-    var_compat e dom (Ref n).
-unfold var_compat; simpl; intros.
-destruct H3 as (Hty,(Hty',Hrec)).
-generalize (Hrec n).
-rewrite H; rewrite H0.
-unfold fcompat; intros.
-apply H3.
-revert H4.
-rewrite <- (H2 _ Hty).
-unfold lift; rewrite int_lift_rec_eq.
-rewrite V.lams0; trivial.
-Qed.
-  Lemma abs_compat : forall e U T M,
-    var_mono e T ->
-    var_equals (push_var e T) M ->
-    typ (T::tenv e) M U ->
-    U <> kind ->
-    var_compat e T (Abs T M).
-unfold var_mono, var_equals, var_compat; intros.
-specialize H with (1:=H3).
-simpl.
-red; intros.
-fold app.
- rewrite beta_eq; try assumption.
- rewrite beta_eq.
- 3:apply H; trivial.
-  apply H0.
-  apply val_push_var; simpl; auto with *.
-  apply in_int_el; apply H; trivial.
-
-  red; red; intros.
-  rewrite H6; reflexivity.
-
- red; red; intros.
- rewrite H6; reflexivity.
-Qed.
-
-  Lemma succ_compat e O :
+  Lemma var_ext_Succ e O :
     typ_ord (tenv e) O ->
     var_mono e O ->
-    var_compat e (NatI O) (SuccI O).
+    var_ext e (NatI O) (SuccI O).
 do 2 red; simpl; intros.
 red in H, H0.
 specialize H0 with (1:=H1).
@@ -778,62 +364,6 @@ rewrite cc_beta_eq; auto with *.
 revert H2; apply TI_mono; auto with *.
  apply H; apply H1.
  apply H; apply H1.
-Qed.
-
-
-  Lemma var_comp_app : forall e dom u v,
-    dom <> kind ->
-    var_compat e dom u ->
-    typ (tenv e) v dom ->
-    var_equals e v ->
-    var_equals e (App u v).
-unfold var_equals; intros.
-simpl.
-transitivity (app (int u i') (int v i)).
- do 2 red in H0.
- apply H0; trivial.
- red in H1.
- specialize H1 with (1:=proj1 H3).
- revert H1; destruct dom; trivial.
- elim H; trivial.
-
- rewrite <- H2 with (1:=H3).
- reflexivity.
-Qed.
-
-
-(** Covariance rules *)
-
-  Lemma var_eq_sub : forall e M, var_equals e M -> var_mono e M.
-unfold var_mono, var_equals; intros.
-apply H in H0.
-rewrite H0; reflexivity.
-Qed.
-
-  Lemma var_mono_ref : forall e n,
-    ords e n = true ->
-    var_mono e (Ref n).
-unfold var_mono; intros.
-destruct H0 as (_,(_,H0)).
-generalize (H0 n); rewrite H.
-simpl; trivial.
-Qed.
-
-  Lemma var_mono_prod : forall e T U,
-    var_equals e T ->
-    var_mono (push_var e T) U ->
-    var_mono e (Prod T U).
-red; simpl; intros.
-specialize (H _ _ H1).
-apply cc_prod_covariant; intros; auto.
- red; red; intros.
- rewrite H3; reflexivity.
-
- apply H0.
- apply val_push_var; auto with *.
-  change (el T i' x).
-  apply in_int_el.
-  rewrite <- H; trivial.
 Qed.
 
   Lemma var_mono_NATi : forall e O,
@@ -901,7 +431,7 @@ Section NatFixRules.
     M (Prod (NatI (OSucc (Ref 1)))
          (lift1 1 (subst_rec (OSucc (Ref 0)) 1 (lift_rec 1 2 U)))).
 
-  Hypothesis stab : var_compat
+  Hypothesis stab : var_ext
     (push_fun (push_ord E (OSucc O)) (NatI (Ref 0)) U)
     (NatI (OSucc (Ref 1)))
     M.
@@ -1078,9 +608,9 @@ rewrite beta_eq.
  apply H; trivial.
 Qed.
 
-  Lemma var_comp_fix :
+  Lemma var_ext_fix :
     var_mono E O ->
-    var_compat E (NatI O) (NatFix O M).
+    var_ext E (NatI O) (NatFix O M).
 intro subO.
 do 2 red; intros.
 assert (isval := proj1 H).
@@ -1216,7 +746,7 @@ apply cc_lam_ext; auto with *.
 
  red; intros.
  rewrite <- H2.
- apply var_comp_fix; trivial.
+ apply var_ext_fix; trivial.
  apply var_eq_sub; trivial.
 Qed.
 
@@ -1224,165 +754,19 @@ End NatFixRules.
 
 Print Assumptions typ_nat_fix.
 
-(****************************************************************************************)
-(** ** Compound judgements : typing + variance *)
-
-Definition typ_inv e M T :=
-  var_equals e M /\ typ (tenv e) M T.
-
-Definition typ_ext e M A B :=
-  var_compat e A M /\ typ (tenv e) M (Prod A B).
-
-Definition typ_mono e M T :=
-  var_mono e M /\ typ (tenv e) M T.
-
-Instance typ_inv_morph e : Proper (eq_term ==> eq_term ==> iff) (typ_inv e).
-apply morph_impl_iff2; auto with *.
-do 4 red; intros.
-destruct H1; split.
- red; intros.
- rewrite <- H; auto.
-
- rewrite <- H; rewrite <- H0; auto.
-Qed.
-
-(** ** Inference rules *)
-
-(** Inclusion relation between judgements *)
-  Lemma typ_inv_mono : forall e M T, typ_inv e M T -> typ_mono e M T.
-destruct 1; split; trivial.
-apply var_eq_sub; trivial.
-Qed.
-
-  Lemma typ_inv_ext : forall e M A B, typ_inv e M (Prod A B) -> typ_ext e M A B.
-destruct 1; split; trivial.
-do 2 red; intros.
-apply H in H1.
-rewrite H1; reflexivity.
-Qed.
-
-(** Subsumption *)
-  Lemma typ_inv_subsumption e M T T' :
-    typ_inv e M T -> sub_typ (tenv e) T T' -> T <> kind -> typ_inv e M T'.
-destruct 1; split; trivial.
-apply typ_subsumption with (2:=H1); trivial.
-Qed.
-
-(** Typing the three kind of variables *)
-  Lemma typ_inv_ref : forall e n T,
-    spec_var e n = false ->
-    nth_error (tenv e) n = value T ->
-    typ_inv e (Ref n) (lift (S n) T).
-intros.
-split.
- apply var_eq_noc; apply noc_var; trivial.
- apply typ_var; trivial.
-Qed.
-
-
-(* Not really useful since (Ref n) should be an ordinal... *)
-  Lemma typ_mono_ref : forall e n T,
-    ords e n = true ->
-    nth_error (tenv e) n = value T ->
-    typ_mono e (Ref n) (lift (S n) T).
-split.
- apply var_mono_ref; trivial.
- apply typ_var; trivial.
-Qed.
-
- Lemma typ_ext_ref e n A B :
-    ords e n = false ->
-    fixs e n = Some A ->
-    A <> kind ->
-    nth_error (tenv e) n = value (Prod A B) ->
-    typ_ext e (Ref n) (lift (S n) A) (lift1 (S n) B).
-split.
- apply var_comp_ref with (2:=H0); trivial.
- reflexivity.
-
- eapply typ_conv.
-  apply typ_var with (1:=H2).
-  2:discriminate.
-
-  unfold lift; rewrite eq_lift_prod; reflexivity.
-Qed.
-
-(** Abstraction *)
-  Lemma typ_inv_abs : forall e U T M,
-    U <> kind ->
-    var_equals e T ->
-    typ_inv (push_var e T) M U ->
-    typ_inv e (Abs T M) (Prod T U).
-destruct 3; split.
- apply var_eq_abs; trivial.
-
- apply typ_abs; trivial.
-Qed.
-
-  Lemma typ_ext_abs : forall e U T M,
-    var_mono e T ->
-    typ_inv (push_var e T) M U ->
-    U <> kind ->
-    typ_ext e (Abs T M) T U.
-destruct 2; split.
- apply abs_compat with U; trivial.
-
- apply typ_abs; trivial.
-Qed.
-
-(** Application *)
-
-  Lemma typ_ext_app : forall e u v A B,
-    A <> kind ->
-    typ_ext e u A B -> 
-    typ_inv e v A ->
-    typ_inv e (App u v) (subst v B).
-intros.
-destruct H0; destruct H1; split.
- apply var_comp_app with (2:=H0); trivial.
-
- apply typ_app with A; trivial.
-Qed.
-
-(** Natural numbers: type and constructors *)
-
-(*
-  Lemma mono_NATi : forall e O,
-    typ_mono e O Ord ->
-    var_mono e (NatI O).
-destruct 1.
-apply var_mono_NATi; auto.
-Qed.
-*)
-(*
-  Lemma mono_OSucc : forall e O o,
-    isOrd o ->
-    typ_mono e O O' ->
-    typ_mono e (OSucc O) (OSucc O').
-destruct 2.
-split.
- apply var_mono_OSucc; trivial.
-
- red; simpl; intros.
- apply lt_osucc_compat; trivial.
- apply H1; trivial.
-Qed.
-*)
-
-  Lemma typ_inv_Zero e O :
+  Lemma typ_eq_Zero e O :
     typ_ord (tenv e) O ->
-(*    var_mono e O -> *)
-    typ_inv e Zero (NatI (OSucc O)).
+    typ_equals e Zero (NatI (OSucc O)).
 split; simpl.
  red; reflexivity.
  apply typ_Zero; trivial.
 Qed.
 
 
-  Lemma typ_inv_Succ e O :
+  Lemma typ_eq_Succ e O :
     typ_ord (tenv e) O ->
     var_equals e O ->
-    typ_inv e (SuccI O) (Prod (NatI O) (NatI (OSucc (lift 1 O)))).
+    typ_equals e (SuccI O) (Prod (NatI O) (NatI (OSucc (lift 1 O)))).
 split; simpl.
  red; simpl; intros.
  apply cc_lam_ext.
@@ -1413,15 +797,15 @@ Qed.
 
 
 (** Case-analysis *)
-  Lemma typ_inv_natcase : forall e O P fZ fS n T,
+  Lemma typ_eq_natcase : forall e O P fZ fS n T,
     typ_ord (tenv e) O ->
     var_mono e O ->
     sub_typ (tenv e) (App P n) T -> 
-    typ_inv e fZ (App P Zero) ->
-    typ_inv (push_var e (NatI O)) fS
+    typ_equals e fZ (App P Zero) ->
+    typ_equals (push_var e (NatI O)) fS
       (App (lift 1 P) (App (SuccI (lift 1 O)) (Ref 0))) ->
-    typ_inv e n (NatI (OSucc O)) ->
-    typ_inv e (Natcase fZ fS n) T.
+    typ_equals e n (NatI (OSucc O)) ->
+    typ_equals e (Natcase fZ fS n) T.
 intros.
 destruct H2.
 destruct H3.
@@ -1444,18 +828,18 @@ Qed.
     typ_ext e (NatFix O M) (NatI O) (subst_rec O 1 U).
 intros e O U M tyO inclO (extM,tyM) tyU.
 split.
- apply var_comp_fix with U; trivial.
+ apply var_ext_fix with U; trivial.
 
  apply typ_nat_fix; trivial.
 Qed.
 
-  Lemma typ_inv_fix : forall e O U M,
+  Lemma typ_eq_fix : forall e O U M,
     typ_ord (tenv e) O ->
     var_equals e O ->
     typ_ext (push_fun (push_ord e (OSucc O)) (NatI (Ref 0)) U) M
       (NatI (OSucc (Ref 1))) (lift1 1 (subst_rec (OSucc (Ref 0)) 1 (lift_rec 1 2 U))) ->
     var_mono (push_var (push_ord e (OSucc O)) (NatI (OSucc (Ref 0)))) U ->
-    typ_inv e (NatFix O M) (Prod (NatI O) (subst_rec O 1 U)).
+    typ_equals e (NatFix O M) (Prod (NatI O) (subst_rec O 1 U)).
 intros e O U M tyO inclO (extM,tyM) tyU.
 split.
  apply var_eq_fix with U; trivial.
@@ -1463,79 +847,20 @@ split.
  apply typ_nat_fix; trivial.
 Qed.
 
-
-
-(** Derived rules for practical examples (basically applies subsumption beforehand) *)
-
-  Lemma typ_inv_ref' : forall e n t T,
-    spec_var e n = false ->
-    nth_error (tenv e) n = value t ->
-    t <> kind ->
-    sub_typ (tenv e) (lift (S n) t) T ->
-    typ_inv e (Ref n) T.
-intros.
-split.
- apply var_eq_noc; apply noc_var; trivial.
-
- apply typ_subsumption with (lift (S n) t); trivial.
-  apply typ_var; trivial.
-
-  destruct t as [(t,tm)|]; simpl in *; auto.
-  discriminate.
-Qed.
-
-  Lemma typ_inv_app : forall e u v V Ur T,
-    V <> kind ->
-    Ur <> kind ->
-    sub_typ (tenv e) (subst v Ur) T ->
-    typ_inv e u (Prod V Ur) ->
-    typ_inv e v V ->
-    typ_inv e (App u v) T.
-intros.
-destruct H2.
-destruct H3.
-split.
- apply var_eq_app; trivial.
-
- apply typ_subsumption with (subst v Ur); trivial.
-  apply typ_app with V; auto.
-
-  destruct Ur as [(Ur,Urm)|]; simpl; trivial.
-  discriminate.
-Qed.
-
-  Lemma typ_inv_rec_call : forall e n x t u T,
-    ords e n = false ->
-    fixs e n = Some t ->
-    t <> kind ->
-    u <> kind ->
-    nth_error (tenv e) n = value (Prod t u) ->
-    sub_typ (tenv e) (subst x (lift1 (S n) u)) T ->
-    typ_inv e x (lift (S n) t) ->
-    typ_inv e (App (Ref n) x) T.
-intros.
-apply typ_inv_subsumption with (2:=H4).
- eapply typ_ext_app with (3:=H5).
-  destruct t as [(t,tm)|]; simpl; trivial; discriminate.
-
-  eapply typ_ext_ref with (4:=H3); trivial.
-
- destruct u as [(u,um)|]; simpl; trivial; discriminate.
-Qed.
-
-  Lemma typ_inv_fix' : forall e O U M T,
+  Lemma typ_eq_fix' : forall e O U M T,
     sub_typ (tenv e) (Prod (NatI O) (subst_rec O 1 U)) T ->
     typ_ord (tenv e) O ->
     var_equals e O ->
     var_mono (push_var (push_ord e (OSucc O)) (NatI (OSucc (Ref 0)))) U ->
     typ_ext (push_fun (push_ord e (OSucc O)) (NatI (Ref 0)) U) M
       (NatI (OSucc (Ref 1))) (lift1 1 (subst_rec (OSucc (Ref 0)) 1 (lift_rec 1 2 U))) ->
-    typ_inv e (NatFix O M) T.
+    typ_equals e (NatFix O M) T.
 intros.
-apply typ_inv_subsumption with (2:=H).
+apply typ_eq_subsumption with (2:=H).
 2:discriminate.
-apply typ_inv_fix; trivial.
+apply typ_eq_fix; trivial.
 Qed.
+
 
 
 (************************************************************************)
@@ -1568,174 +893,148 @@ Definition nat_ind K :=
         (Ref 0)))))).
 
 Lemma nat_ind_def e K (cK:forall f, noccur(B.cons false f)K) :
-  typ_inv e (nat_ind K) (nat_ind_typ K).
+  typ_equals e (nat_ind K) (nat_ind_typ K).
 assert (eq_term Nat (NatI Infty)).
  red; simpl.
  red; unfold NAT; reflexivity.
 unfold nat_ind, nat_ind_typ.
-apply typ_inv_abs; try discriminate.
- apply var_eq_noc; noc_tac.
- trivial.
-(* *)
-apply typ_inv_abs; try discriminate.
- apply var_eq_noc; noc_tac.
-(* *)
-apply typ_inv_abs; try discriminate.
- apply var_eq_noc; noc_tac.
-(* *)
-assert (e1 : eq_term (App (Ref 3) (Ref 0)) (subst_rec Infty 1 (App (Ref 4) (Ref 0)))).
- simpl.
- red; intros.
- unfold V.lams, V.shift; simpl.
- apply cc_app_morph; apply H0.
-rewrite e1.
-apply typ_inv_fix; auto.
- (* infty : infty *)
- apply typ_Infty.
- red; reflexivity.
-
- (* codom mono *)
- Focus 2.
- apply var_eq_sub.
- apply var_eq_noc.
- noc_tac.
-
- (* fix body *)
- apply typ_ext_abs; try discriminate.
-  apply var_mono_NATi.
-   apply typ_OSucc.
-   apply typ_ord_ref with (OSucc Infty); auto.
-    discriminate.
-    red; simpl; auto.
-
-   apply var_mono_OSucc.
-   apply var_mono_ref; reflexivity.
-
-  apply typ_inv_natcase with (Ref 2) (Ref 5); auto.
-   eapply typ_ord_ref.
-    simpl; reflexivity.
-    discriminate.
-    red; simpl; auto.
-
-   apply var_mono_ref; simpl; reflexivity.
-
-   (* eqtrm *)
-   simpl tenv; apply sub_refl.
-   red; simpl; intros; reflexivity.
-
-   (* branch 0 *)
-   eapply typ_inv_ref'.
-    compute; reflexivity.
-    simpl; reflexivity.
-    discriminate.
-
-    (* eqtrm *)
-    apply sub_refl; red; simpl; intros.
-    unfold V.lams, V.shift; simpl; reflexivity.
-
-   (* branch S *)
-   apply typ_inv_app with (App (Ref 6) (Ref 0))
-     (App (Ref 7) (App (SuccI Infty) (Ref 1))); try discriminate.
-    simpl tenv.
-    apply sub_refl; red; intros; simpl.
-    (* conversion (succ domain) *)
-    unfold V.lams, V.shift; simpl.
-    assert (i 0 ∈ NATi (i 3)).
-     generalize (H0 0 _ (eq_refl _)); simpl.
-     unfold V.lams, V.shift; simpl; trivial.
-    rewrite beta_eq.
-     rewrite beta_eq; auto with *.
-     red; intros; apply inr_morph; trivial.
-
-      red; intros; apply inr_morph; trivial.
-
-     apply NATi_NAT in H1; trivial.
-     generalize (H0 3 _ (eq_refl _)); simpl; intro.
-     apply isOrd_inv with (osucc omega); auto.
-
-    (**)
-    apply typ_inv_app with (NatI Infty)
-      (Prod (App (Ref 7) (Ref 0)) (App (Ref 8) (App (SuccI Infty) (Ref 1))));
-      try discriminate.
-     (* eqtrm *)
-     apply sub_refl; red; intros; simpl.
-     unfold V.lams, V.shift; simpl.
-     reflexivity.
-
-     eapply typ_inv_ref'.
-      compute; reflexivity.
-      simpl; reflexivity.
-      discriminate.
-
-      (* eqtrm *)
-      apply sub_refl; red; intros; simpl.
-      unfold V.shift, V.lams, V.shift; simpl.
-      reflexivity.
-
-     eapply typ_inv_ref'.
-      compute; reflexivity.
-      simpl; reflexivity.
-      discriminate.
-
-      (* subtyping: nat -> infty *)
-      red; simpl; intros.
-      unfold V.lams, V.shift in H1; simpl in H1.
-      apply NATi_NAT in H1; trivial.
-      generalize (H0 3 _ (eq_refl _)); simpl; intro.
-      apply isOrd_inv with (osucc omega); auto.
-
-    (**)
-    eapply typ_inv_rec_call.
-     compute; trivial.
-     simpl; reflexivity.
-     discriminate.
-     2:simpl; reflexivity.
-     discriminate.
-
-     (* eqtrm *)
-     apply sub_refl; red; intros; simpl.
-     unfold V.lams, V.shift; simpl.
-     reflexivity.
-
-     eapply typ_inv_ref'.
-      compute; reflexivity.
-      simpl; reflexivity.
-      discriminate.
-
-      (* eqtrm *)
-      apply sub_refl; red; intros; simpl.
-      reflexivity.
-
-   (* Scrutinee *)
-   eapply typ_inv_ref'.
-    compute; reflexivity.
-    simpl; reflexivity.
-    discriminate.
-
-    (* eqtrm *)
-    apply sub_refl; red; intros; simpl.
-    reflexivity.
-Qed.
-
-(*
-Lemma int_abs_eq : forall T M i i',
-  int T i == int T i' ->
-  (forall x, x ∈ int T i -> int M (V.cons x i) == int M (V.cons x i')) ->
-  int (Abs T M) i == int (Abs T M) i'.
-intros.
-simpl.
-apply cc_lam_ext.
- trivial.
-red; intros.
-transitivity (int M (V.cons x' i)).
- apply int_morph; auto with *.
- apply V.cons_morph; trivial.
+apply typ_eq_abs with (s1:=kind); try discriminate; auto.
  reflexivity.
 
- apply H0.
- rewrite <- H2; trivial.
+ split.
+  apply var_eq_noc; noc_tac.
+  trivial.
+
+  red; simpl; trivial.
+(* *)
+apply typ_eq_abs with (s1:=kind); try discriminate; auto.
+ reflexivity.
+
+ split.
+  apply var_eq_noc; noc_tac.
+  red; simpl; trivial.
+(* *)
+apply typ_eq_abs with (s1:=kind); try discriminate; auto.
+ reflexivity.
+
+ split.
+  apply var_eq_noc; noc_tac.
+  red; simpl; trivial.
+(* *)
+apply typ_eq_fix' with (U:=App (Ref 4) (Ref 0)); auto.
+ red; simpl; intros.
+ exact H1.
+ (* Infty : ord *)
+ apply typ_Infty.
+ (* Infty mono *)
+ apply var_eq_noc; noc_tac.
+ (* codom mono *)
+ apply var_eq_sub; apply var_eq_noc; noc_tac.
+(* fix body *)
+apply typ_ext_abs; try discriminate.
+ split;[|red;simpl;trivial].
+ apply var_mono_NATi.
+  apply typ_OSucc.
+  apply typ_ord_ref with (OSucc Infty); auto.
+   discriminate.
+   red; simpl; auto.
+
+  apply var_mono_OSucc.
+  apply var_mono_ref; reflexivity.
+(* case *)
+apply typ_eq_natcase with (Ref 2) (Ref 5); auto.
+ eapply typ_ord_ref.
+  simpl; reflexivity.
+  discriminate.
+  red; simpl; auto.
+
+ apply var_mono_ref; simpl; reflexivity.
+
+ (* sub *)
+ simpl tenv; apply sub_refl.
+ red; simpl; intros; reflexivity.
+
+ (* branch 0 *)
+ eapply typ_eq_ref'.
+  compute; reflexivity.
+  simpl; reflexivity.
+  discriminate.
+ (* eqtrm *)
+ red; intros; exact H1.
+
+ (* branch S *)
+ apply typ_eq_app with (App (Ref 6) (Ref 0))
+   (App (Ref 7) (App (SuccI Infty) (Ref 1))); try discriminate.
+  simpl tenv.
+  apply sub_refl; red; intros; simpl.
+  (* conversion (succ domain) *)
+  unfold V.lams, V.shift; simpl.
+  assert (i 0 ∈ NATi (i 3)).
+   generalize (H0 0 _ (eq_refl _)); simpl.
+   unfold V.lams, V.shift; simpl; trivial.
+  rewrite beta_eq.
+   rewrite beta_eq; auto with *.
+   red; intros; apply inr_morph; trivial.
+
+    red; intros; apply inr_morph; trivial.
+
+   apply NATi_NAT in H1; trivial.
+   generalize (H0 3 _ (eq_refl _)); simpl; intro.
+   apply isOrd_inv with (osucc omega); auto.
+
+  (**)
+  apply typ_eq_app with (NatI Infty)
+    (Prod (App (Ref 7) (Ref 0)) (App (Ref 8) (App (SuccI Infty) (Ref 1))));
+    try discriminate.
+   (* eqtrm *)
+   red; simpl; intros.
+   exact H1.
+
+   eapply typ_eq_ref'.
+    compute; reflexivity.
+    simpl; reflexivity.
+    discriminate.
+    (* eqtrm *)
+    red; simpl; intros; assumption.
+
+   eapply typ_eq_ref'.
+    compute; reflexivity.
+    simpl; reflexivity.
+    discriminate.
+    (* subtyping: nat -> infty *)
+    red; simpl; intros.
+    unfold V.lams, V.shift in H1; simpl in H1.
+    apply NATi_NAT in H1; trivial.
+    generalize (H0 3 _ (eq_refl _)); simpl; intro.
+    apply isOrd_inv with (osucc omega); auto.
+
+  (**)
+  eapply typ_ext_app.
+   compute; trivial.
+   simpl; reflexivity.
+   discriminate.
+   discriminate.
+   2:simpl; reflexivity.
+   discriminate.
+   (* eqtrm *)
+   red; simpl; intros; assumption.
+
+   eapply typ_eq_ref'.
+    compute; reflexivity.
+    simpl; reflexivity.
+    discriminate.
+    (* eqtrm *)
+    red; simpl; intros; assumption.
+
+ (* Scrutinee *)
+ eapply typ_eq_ref'.
+  compute; reflexivity.
+  simpl; reflexivity.
+  discriminate.
+  (* eqtrm *)
+  red; simpl; intros; assumption.
 Qed.
-*)
+
 
 (** Subtraction *)
 
@@ -1759,23 +1058,22 @@ Definition minus_typ O := Prod (NatI O) (Prod (NatI Infty) (NatI (lift 2 O))).
 Lemma minus_def e O :
   typ_ord (tenv e) O ->
   var_equals e O ->
-  typ_inv e (minus O) (minus_typ O).
+  typ_equals e (minus O) (minus_typ O).
 intros tyO eqO.
 unfold minus, minus_typ.
-apply typ_inv_fix' with (Prod (NatI Infty) (NatI (Ref 2))); auto.
+apply typ_eq_fix' with (Prod (NatI Infty) (NatI (Ref 2))); auto.
  (* sub *)
+ rewrite eq_subst_prod.
  apply sub_refl.
  apply eq_typ_prod.
   reflexivity.
+ apply eq_typ_prod.
+  red; intros; simpl; reflexivity.
 
-  rewrite eq_subst_prod.
-  apply eq_typ_prod.
-   red; intros; simpl; reflexivity.
-
-   red; intros; simpl.
-   unfold lift; rewrite int_lift_rec_eq.
-   rewrite V.lams0.
-   unfold V.lams, V.shift; simpl; reflexivity.
+  red; intros; simpl.
+  unfold lift; rewrite int_lift_rec_eq.
+  rewrite V.lams0.
+  unfold V.lams, V.shift; simpl; reflexivity.
 
  (* codom mono *)
  apply var_mono_prod.
@@ -1794,6 +1092,7 @@ apply typ_inv_fix' with (Prod (NatI Infty) (NatI (Ref 2))); auto.
 
  (* fix body *)
  apply typ_ext_abs; try discriminate.
+  split;[|red;simpl; trivial].
   apply var_mono_NATi.
    apply typ_OSucc.
    eapply typ_ord_ref.
@@ -1811,22 +1110,18 @@ apply typ_inv_fix' with (Prod (NatI Infty) (NatI (Ref 2))); auto.
  rewrite eq_lift_prod.
  rewrite eq_subst_prod.
  unfold lift1; rewrite eq_lift_prod.
- eapply typ_inv_subsumption.
- apply typ_inv_abs.
- 5:discriminate.
-  Focus 4.
-  apply sub_refl.
-  apply eq_typ_prod.
-   red; intros; simpl; reflexivity.
-
-   reflexivity.
-
+ eapply typ_eq_subsumption.
+ apply typ_eq_abs with (s1:=kind); try discriminate; auto.
+  6:discriminate.
+  5:apply sub_refl; reflexivity.
   discriminate.
+  red; intros; simpl; reflexivity.
 
+  split;[|red;simpl;trivial].
   apply var_eq_noc; noc_tac.
 
  (**)
- apply typ_inv_natcase with (Ref 3)
+ apply typ_eq_natcase with (Ref 3)
     (Abs (NatI (OSucc (Ref 3))) (NatI (OSucc (Ref 4)))); auto.
   eapply typ_ord_ref.
    simpl; reflexivity.
@@ -1851,8 +1146,8 @@ apply typ_inv_fix' with (Prod (NatI Infty) (NatI (Ref 2))); auto.
    red; simpl; reflexivity.
 
   (* branch 0 *)
-  eapply typ_inv_subsumption.
-   apply typ_inv_Zero.
+  eapply typ_eq_subsumption.
+   apply typ_eq_Zero.
    eapply typ_ord_ref with (n:=3).
     simpl; reflexivity.
     discriminate.
@@ -1873,7 +1168,7 @@ apply typ_inv_fix' with (Prod (NatI Infty) (NatI (Ref 2))); auto.
      apply typ_OSucc; trivial.
 
   (* branch S *)
-  apply typ_inv_natcase with Infty
+  apply typ_eq_natcase with Infty
      (Abs (NatI (OSucc Infty)) (NatI (OSucc (Ref 5)))); auto.
    apply typ_Infty.
 
@@ -1910,7 +1205,7 @@ apply typ_inv_fix' with (Prod (NatI Infty) (NatI (Ref 2))); auto.
     revert H0; apply TI_incl; auto with *.
 
   (* branch 0 *)
-  eapply typ_inv_ref'.
+  eapply typ_eq_ref'.
    compute; reflexivity.
    simpl; reflexivity.
    discriminate.
@@ -1925,7 +1220,7 @@ apply typ_inv_fix' with (Prod (NatI Infty) (NatI (Ref 2))); auto.
     apply typ_Infty.
 
   (* branch S *)    
-  apply typ_inv_app with (NatI Infty) (NatI (Ref 6)).
+  apply typ_eq_app with (NatI Infty) (NatI (Ref 6)).
    discriminate.
    discriminate.
 
@@ -1961,9 +1256,10 @@ apply typ_inv_fix' with (Prod (NatI Infty) (NatI (Ref 2))); auto.
      red; intros; simpl.
      reflexivity.
 
-   eapply typ_inv_rec_call.
+   eapply typ_ext_app.
     compute; reflexivity.
     simpl; reflexivity.
+    discriminate.
     discriminate.
     2:simpl; reflexivity.
     discriminate.
@@ -1973,7 +1269,7 @@ apply typ_inv_fix' with (Prod (NatI Infty) (NatI (Ref 2))); auto.
     rewrite eq_subst_prod.
     red; intros; simpl; reflexivity.
 
-    eapply typ_inv_ref'.
+    eapply typ_eq_ref'.
      compute; reflexivity.
      simpl; reflexivity.
      discriminate.
@@ -1981,7 +1277,7 @@ apply typ_inv_fix' with (Prod (NatI Infty) (NatI (Ref 2))); auto.
      apply sub_refl.
      red; intros; simpl; reflexivity.
 
-     eapply typ_inv_ref'.
+     eapply typ_eq_ref'.
       compute; reflexivity.
       simpl; reflexivity.
       discriminate.
@@ -1990,17 +1286,16 @@ apply typ_inv_fix' with (Prod (NatI Infty) (NatI (Ref 2))); auto.
       red; intros; simpl; reflexivity.
 
    (**)
-   eapply typ_inv_ref'.
+   eapply typ_eq_ref'.
     compute; reflexivity.
     simpl; reflexivity.
     discriminate.
-
     (* infty < infty+ *)
     red; simpl; intros.
     revert H0; apply TI_incl; auto with *.
 
   (**)
-  eapply typ_inv_ref'.
+  eapply typ_eq_ref'.
    compute; reflexivity.
    simpl; reflexivity.
    discriminate.
