SN_NAT.v
@@ -59,338 +59,55 @@ rewrite Real_def; intros; trivial.
  apply cNAT_morph; trivial.
 Qed.
 
-  Notation "[ x , t ] \real A" := (x ∈ El A  /\ inSAT t (Real A x)) (at level 60).
-
-Lemma realNat_def : forall i n t,
-  [n,t] \real int Nat i <-> n ∈ cc_bot NAT' /\ inSAT t (cNAT n).
-intros.
-rewrite ElNat_eq.
-split; destruct 1; split; trivial.
- rewrite RealNat_eq in H0; trivial.
- rewrite RealNat_eq; trivial.
-Qed.
-
 (** Typing rules of constructors *)
 Lemma typ_0 : forall e, typ e Zero Nat.
 intros.
 apply typ_common;[exact I|intros].
-apply realNat_def; split.
+apply and_split; intros.
+ red; rewrite ElNat_eq.
  apply cc_bot_intro; apply ZERO_typ'.
 
+ red in H0; rewrite ElNat_eq in H0.
+ rewrite RealNat_eq; trivial.
  apply cNAT_ZE.
 Qed.
-
-Lemma sn_SU : Lc.sn SU.
-unfold SU.
-constructor; intros ? h.
-apply nf_norm in h;[contradiction|repeat constructor].
-Qed.
-
 
 Lemma typ_S : forall e, typ e Succ (Prod Nat (lift 1 Nat)).
 intros.
 apply typ_common;[exact I|intros i j isval].
-rewrite intProd_eq.
-apply prod_intro_sn.
- red; intros.
- rewrite H0; reflexivity.
+apply and_split; intros.
+ red.
+ rewrite El_int_prod.
+ apply cc_prod_intro.
+  do 2 red; intros.
+  rewrite H0; reflexivity.
 
- red; intros.
- rewrite H0; reflexivity.
+  do 2 red; intros.
+  rewrite H0; reflexivity.
 
- apply sn_SU.
-
- destruct 1.
- red in H; rewrite ElNat_eq in H.
- apply and_split; intros.
-  red; rewrite int_cons_lift_eq.
-  rewrite ElNat_eq.
+  intros.
+  rewrite int_cons_lift_eq.
+  rewrite ElNat_eq in H|-*.
   apply cc_bot_intro; apply SUCC_typ'; trivial.
 
-  red in H1.
-  rewrite int_cons_lift_eq in H1|-*.
-  rewrite ElNat_eq in H1.
-  rewrite RealNat_eq in H0|-*; trivial.
-  apply cNAT_SU; trivial.
-Qed.
-
-Lemma typ_N : forall e, typ e Nat kind.
-red; red; simpl; intros.
-split;[discriminate|].
-split.
- red.
- exists List.nil.
- exists Nat.
-  reflexivity.
-
-  exists empty.
-  simpl; intros _.
-  unfold SN_CC_Model.inX; rewrite El_def.
-  apply union2_intro1; apply singl_intro.
-
- exact Lc.sn_K.
-Qed.
-
-Require Import ZFord ZFfix.
-Require Import ZFfixrec.
-
-Definition NREC f g n y :=
-  forall (P:set->set->Prop),
-  Proper (eq_set==>eq_set==>iff) P ->
-  P empty empty ->
-  P ZERO f ->
-  (forall m z, m ∈ cc_bot NAT' -> P m z -> P (SUCC m) (g m z)) ->
-  P n y.
-
-Lemma NREC_mt f g : NREC f g empty empty.
-red; intros; trivial.
-Qed.
-Lemma NREC_ZERO f g : NREC f g ZERO f.
-red; intros; trivial.
-Qed.
-Lemma NREC_SUCC f g n y:
-  n ∈ cc_bot NAT' -> NREC f g n y -> NREC f g (SUCC n) (g n y).
-unfold NREC; intros.
-apply H4; trivial.
-apply H0; trivial.
-Qed.
-Instance NREC_morph :
-  Proper (eq_set==>(eq_set==>eq_set==>eq_set)==>eq_set==>eq_set==>iff) NREC.
-apply morph_impl_iff4; auto with *.
-unfold NREC; do 6 red; intros.
-rewrite <- H in H6.
-rewrite <- H1; rewrite <- H2; apply H3; trivial.
-intros.
-rewrite (H0 _ _ (reflexivity m) _ _ (reflexivity z)).
-auto.
-Qed.
-Instance NREC_morph_eq :
-  Proper (eq_set==>eq==>eq_set==>eq_set==>iff) NREC.
-apply morph_impl_iff4; auto with *.
-unfold NREC; do 6 red; intros.
-subst x0; rewrite <- H in H6.
-rewrite <- H1; rewrite <- H2; apply H3; trivial.
-Qed.
-
-Lemma NREC_inv f g n y :
-  NREC f g n y ->
-   NREC f g n y /\
-   ((n==empty/\y==empty) \/
-    (n==ZERO/\y==f) \/
-    (exists2 m, n == SUCC m & exists2 z, NREC f g m z & y==g m z)).
-intros H; apply H; intros.
- do 3 red; intros.
- apply and_iff_morphism.
-  apply NREC_morph_eq; auto with *.
-
-  repeat apply or_iff_morphism.
-   rewrite H0; rewrite H1; reflexivity.
-   rewrite H0; rewrite H1; reflexivity.
-   apply ex2_morph; red; intros.
-    rewrite H0; reflexivity.
-   apply ex2_morph; red; intros.
-    apply NREC_morph_eq; auto with *.
-    rewrite H1; reflexivity.
-
- split; auto with *.
- apply NREC_mt.
-
- split; auto with *.
- apply NREC_ZERO.
-
- destruct H1 as (?,_).
- split.
-  apply NREC_SUCC; trivial.
-
-  right; right.
-  exists m;[reflexivity|].
-  exists z; auto with *.
-Qed.
-Lemma NREC_inv_mt f g y :
-  NREC f g empty y -> y == empty.
-intros; apply NREC_inv in H;
-   destruct H as (_,[(_,eqy)|[(abs,_)|(n,abs,_)]]); auto.
- apply discr_mt_pair in abs; contradiction.
- apply discr_mt_pair in abs; contradiction.
-Qed.
-Lemma NREC_inv_ZERO f g y :
-  NREC f g ZERO y -> y == f.
-intros; apply NREC_inv in H;
-   destruct H as (_,[(abs,_)|[(_,eqy)|(n,abs,_)]]); auto.
- symmetry in abs; apply discr_mt_pair in abs; contradiction.
- apply NATf_discr in abs; contradiction.
-Qed.
-Lemma NREC_inv_SUCC f g n y :
-  morph2 g ->
-  NREC f g (SUCC n) y -> exists2 z, NREC f g n z & y == g n z.
-intros; apply NREC_inv in H0;
-   destruct H0 as (_,[(abs,_)|[(abs,_)|(m,eqS,(z,defz,eqy))]]).
- symmetry in abs; apply discr_mt_pair in abs; contradiction.
- symmetry in abs; apply NATf_discr in abs; contradiction.
-
- apply SUCC_inj in eqS.
- rewrite <- eqS in defz, eqy; eauto.
-Qed.
-
-Require Import ZFrepl.
-
-Lemma NAT'_ind P n :
-  Proper (eq_set==>iff) P ->
-  n ∈ cc_bot NAT' ->
-  P empty ->
-  P ZERO ->
-  (forall m, m ∈ cc_bot NAT' -> P m -> P (SUCC m)) -> 
-  P n.
-intros.
-revert n H0; unfold NAT'; apply isOrd_ind with (2:=isOrd_omega); intros.
-apply cc_bot_ax in H6; destruct H6.
- rewrite H6; trivial.
-
- apply TI_elim in H6; auto with *.
- destruct H6 as (o',o'o,?).
- apply NATf_case with (3:=H6); intros.
-  rewrite H7; trivial.
-
-  rewrite H8; apply H3.
-   revert H7; apply cc_bot_mono.
-   apply NATf'_stages.
-   apply isOrd_inv with y; trivial.
-
-   apply H5 with o'; trivial. 
-Qed.
-
-Lemma NREC_uch_mt f g :
-  uchoice_pred (NREC f g empty).
-split;[|split]; intros.
- rewrite <- H; trivial.
-
- exists empty; apply NREC_mt.
- apply NREC_inv_mt in H.
- apply NREC_inv_mt in H0.
- rewrite H; rewrite H0; reflexivity.
-Qed.
-
-Lemma NREC_uch_ZERO f g :
-  uchoice_pred (NREC f g ZERO).
-split;[|split]; intros.
- rewrite <- H; trivial.
-
- exists f; apply NREC_ZERO.
- apply NREC_inv_ZERO in H.
- apply NREC_inv_ZERO in H0.
- rewrite H; rewrite H0; reflexivity.
-Qed.
-
-Lemma NREC_uch f g n :
-  morph2 g ->
-  n ∈ cc_bot NAT' ->
-  uchoice_pred (NREC f g n).
-intros gm tyn.
-apply NAT'_ind with (2:=tyn).
- do 2 red; intros; apply uchoice_pred_morph.
- red; intros; apply NREC_morph_eq; auto with *.
-
- apply NREC_uch_mt.
-
- apply NREC_uch_ZERO.
-
- intros m tym (_,((z,?),muniq)).
- split; [|split]; intros.
-  rewrite <- H0; trivial.
-
-  exists (g m z); apply NREC_SUCC; trivial.
-
-  apply NREC_inv_SUCC in H0; trivial.
-  apply NREC_inv_SUCC in H1; trivial.
-  destruct H0 as (y,?,eqx).
-  destruct H1 as (y',?,eqx').
-  rewrite eqx; rewrite eqx'; apply gm; eauto with *.
-Qed.
-
-Definition NAT_RECT f g n := uchoice (NREC f g n).
-
-Instance NAT_RECT_morph :
-  Proper (eq_set==>(eq_set==>eq_set==>eq_set)==>eq_set==>eq_set) NAT_RECT.
-do 4 red; intros.
-apply uchoice_morph_raw.
-red; intros; apply NREC_morph; trivial.
-Qed.
-Instance NAT_RECT_morph_eq :
-  Proper (eq_set==>eq==>eq_set==>eq_set) NAT_RECT.
-do 4 red; intros.
-apply uchoice_morph_raw.
-red; intros; apply NREC_morph_eq; trivial.
-Qed.
-
-Lemma NAT_RECT_mt f g :
-  NAT_RECT f g empty == empty.
-symmetry; apply uchoice_ext.
- apply NREC_uch_mt.
-
- apply NREC_mt.
-Qed.
-
-Lemma NAT_RECT_ZERO f g :
-  NAT_RECT f g ZERO == f.
-symmetry; apply uchoice_ext.
- apply NREC_uch_ZERO.
-
- apply NREC_ZERO.
-Qed.
-
-Lemma NAT_RECT_eq f g n y :
-  morph2 g ->
-  n ∈ cc_bot NAT' ->
-  (NAT_RECT f g n == y <-> NREC f g n y).
-intros.
-assert (ch := NREC_uch f H H0).
-assert (eqn := uchoice_def _ ch).
-split; intros.
- rewrite <- H1; trivial.
-
- symmetry; apply uchoice_ext; trivial.
-Qed.
-
-Lemma NAT_RECT_SUCC f g n :
-  morph2 g ->
-  n ∈ cc_bot NAT' ->
-  NAT_RECT f g (SUCC n) == g n (NAT_RECT f g n).
-intros.
-apply NAT_RECT_eq; trivial.
- apply cc_bot_intro.
- apply SUCC_typ'; trivial.
-
- apply NREC_SUCC; trivial.
-
- apply NAT_RECT_eq; trivial.
- reflexivity.
-Qed.
-
-
-Lemma NAT_RECT_typ f g n P :
-  morph1 P ->
-  n ∈ cc_bot NAT' ->
-  empty ∈ P empty ->
-  f ∈ P ZERO ->
-  g ∈ cc_prod (cc_bot NAT') (fun m => cc_arr (P m) (P (SUCC m))) ->
-  NAT_RECT f (fun m y => cc_app (cc_app g m) y) n ∈ P n.
-intros.
-apply NAT'_ind with (2:=H0).
- do 2 red; intros.
- apply in_set_morph; auto.  
- apply NAT_RECT_morph_eq; auto with *.
-
- rewrite NAT_RECT_mt; trivial.
-
- rewrite NAT_RECT_ZERO; trivial.
-
+ red in H.
+ rewrite El_int_prod in H.
+ rewrite Real_int_prod; trivial.
+ apply piSAT0_intro'.
+ 2:exists empty; auto.
  intros.
- rewrite NAT_RECT_SUCC; trivial.
-  apply cc_prod_elim with (2:=H4) in H3.
-  apply cc_arr_elim with (1:=H3) (2:=H5).
+ rewrite int_cons_lift_eq.
+ rewrite ElNat_eq in H0.
+ simpl (int Succ i); rewrite beta_eq.
+  rewrite RealNat_eq in H1|-*; trivial.
+   apply cNAT_SU; trivial.
 
-  do 3 red; intros.
-  rewrite H6; rewrite H7; reflexivity.
+   apply cc_bot_intro; simpl.
+   apply SUCC_typ'; trivial.
+
+  red; intros; apply couple_morph; auto with *.
+
+  red; rewrite El_def; trivial.
 Qed.
 
 (** Recursor *)
@@ -443,19 +160,6 @@ rewrite ElNat_eq in tyn.
 rewrite RealNat_eq in satn; trivial.
 rewrite El_int_prod in tyg.
 rewrite Real_int_prod in satg; trivial.
-(*assert (tygg :forall k h : set,
-   k ∈ cc_bot NAT' -> h ∈ El (app (int P i) k) -> gg k h ∈ El (app (int P i) (SUCC k))).
- intros.
- rewrite <- ElNat_eq with (i:=i) in H.
- apply cc_prod_elim with (2:=H) in tyg.
- rewrite El_int_prod in tyg.
- assert (tyh : h ∈ El (app (int (lift 1 P) (V.cons k i)) k)).
-  rewrite int_cons_lift_eq; trivial.
- apply cc_prod_elim with (2:=tyh) in tyg.
- simpl in tyg.
- rewrite int_lift_eq in tyg.
- rewrite beta_eq in tyg; auto with *.
- red; intros; apply succ_morph; trivial.*)
 assert (NRtyp : forall n, n ∈ cc_bot NAT' ->
   NAT_RECT (int f i) gg n ∈ El (app (int P i) n)).
  intros.
@@ -496,21 +200,6 @@ apply and_split; intros.
 
   rewrite NAT_RECT_ZERO; trivial.
 
-Lemma interSAT_mono_subset :
-  forall A (P Q:A->Prop) (F:sig P->SAT) (G:sig Q->SAT),
-  (forall x, Q x -> P x) ->
-  (forall x Px Qx,
-   inclSAT (F (exist P x Px)) (G (exist Q x Qx))) ->
-  inclSAT (interSAT F) (interSAT G).
-red; intros.
-split.
- apply sat_sn in H1; trivial.
-intros (x,Qx).
-change (inSAT t (G (exist Q x Qx))).
-apply H0 with (Px:=H _ Qx).
-apply interSAT_elim with (1:=H1).
-Qed.
-
   revert satg; apply interSAT_mono_subset; simpl proj1_sig; intros.
    rewrite ElNat_eq; trivial.
   apply prodSAT_mono.
@@ -518,25 +207,9 @@ Qed.
    rewrite RealNat_eq; auto with *.
   apply cc_prod_elim with (2:=Px) in tyg.
   rewrite El_int_prod in tyg.
-Instance inclSAT_morph : Proper (eqSAT==>eqSAT==>iff) inclSAT.
-apply morph_impl_iff2; auto with *.
-do 5 red; intros.
- rewrite <- H0; rewrite <- H in H2; auto. 
-Qed.
   rewrite Real_int_prod; trivial.
 
-Lemma incl_interSAT_l A (F:A->SAT) x :
-  inclSAT (interSAT F) (F x).
-red; intros.
-apply interSAT_elim with (1:=H).
-Qed.
-
   red; intros.
-Lemma depSAT_elim' A (P:A->Prop) F t :
-  inSAT t (depSAT P F) -> id (forall x, P x -> inSAT t (F x)).
-red; intros.
-apply depSAT_elim with (1:=H) (2:=H0).
-Qed.
   apply depSAT_elim' in H0; red in H0.
   specialize H0 with (x0:=NAT_RECT (int f i) gg x).
   change (int (App (lift 1 P) (Ref 0)) (V.cons x i)) with
