SN_W.v
@@ -16,6 +16,10 @@ Import Sat Sat.SatSet.
 
 Require Import SN_ord.
 
+(** Judgments with variance *)
+
+Require Import SN_variance.
+
 (** W *)
 
 Lemma val_ok_cons_default e T i j :
@@ -88,6 +92,15 @@ apply sigma_morph.
   apply cc_bot_morph; auto with *.
 Qed.
 
+  Lemma WF'mono i : Proper (incl_set==>incl_set) (WF' i).
+do 2 red; intros.
+unfold WF'.
+apply W_F_mono.
+ do 2 red; intros; apply Bw_morph; auto with *.
+ apply cc_bot_mono; trivial.
+Qed.
+  Hint Resolve WF'mono.
+
 Instance RW_morph : Proper (eq_val ==> eq_set ==> eq_set ==> eqSAT) RW.
 do 4 red; intros.
 unfold RW.
@@ -96,6 +109,18 @@ apply rWi_morph_gen; auto with *.
  apply Bw_morph; trivial.
  apply RAw_morph; trivial.
  apply RBw_morph; trivial.
+Qed.
+
+Lemma TI_inv i x :
+  isOrd o ->
+  x ∈ TI (WF' i) o ->
+  exists2 o', o' ∈ o & x ∈ TI (WF' i) (osucc o').
+intros.
+apply TI_elim in H0; auto.
+destruct H0.
+exists x0; trivial.
+rewrite TI_mono_succ; trivial.
+apply isOrd_inv with o; trivial.
 Qed.
 
 Definition WI (O:trm) : trm.
@@ -206,7 +231,6 @@ left; exists (fun i => couple (int x i) (int f i))
 Defined.
 
 
-
 Lemma typ_Wc : forall O X F,
   typ e O (Ordt o) ->
   typ e X A ->
@@ -223,20 +247,17 @@ destruct tyord_inv with (3:=H)(4:=H2) as (?,(?,_)); trivial.
 apply in_int_intro; try discriminate.
 assert (couple (int X0 i) (int F i) ∈ TI (WF' i) (osucc (int O i))).
  apply TI_intro with (int O i); auto.
-  apply WF'_morph; reflexivity.
+ apply couple_intro_sigma.
+  do 2 red; intros.
+  rewrite H6; reflexivity.
 
-  unfold W_F.
-  apply couple_intro_sigma.
-   do 2 red; intros.
-   rewrite H6; reflexivity.
+  apply H0.
 
-   apply H0.
-
-   destruct H1.
-   red in H1; rewrite El_int_arr in H1.
-   rewrite El_int_W in H1.
-   rewrite <- int_subst_eq in H1.
-   trivial.
+  destruct H1.
+  red in H1; rewrite El_int_arr in H1.
+  rewrite El_int_W in H1.
+  rewrite <- int_subst_eq in H1.
+  trivial.
 split.
  red; rewrite El_int_W; auto.
 
@@ -355,8 +376,6 @@ apply and_split; intros.
   apply discr_mt_pair.   
 
   simpl in H1; rewrite TI_mono_succ in H1; auto with *.
-  2:apply W_F'_mono; trivial.
-  2:apply Bw_morph; reflexivity.
   assert (fst (int n i) ∈ Aw i).
    apply fst_typ_sigma in H1; trivial.
   assert (snd (int n i) ∈ cc_arr (Bw i (fst (int n i))) (cc_bot (TI (WF' i) (int O i)))).
@@ -471,6 +490,7 @@ apply typ_Wcase with O; trivial.
 Qed.
 
 End Wtypes_typing.
+Hint Resolve WF'mono.
 
 Lemma typ_WI_type n eps e A B O :
   isOrd eps ->
@@ -548,474 +568,6 @@ apply and_split; intros.
  apply Lc.sn_abs; trivial.
 Qed.
 
-(********************************************************************************)
-(** Occurrences *)
-
-
-  (* Non-occurrence : interp do not depend on variables in set [f] *)
-  Definition noccur (f:nat->bool) (T:trm) : Prop :=
-    forall i i',
-    (forall n, if f n then True else i n == i' n) ->
-    int T i == int T i'.
-
-  Lemma noc_var : forall f n, f n = false -> noccur f (Ref n).
-red; simpl; intros.
-specialize (H0 n).
-rewrite H in H0; trivial.
-Qed.
-
-  Lemma noc_kind : forall f, noccur f kind.
-red; simpl; reflexivity.
-Qed.
-
-  Lemma noc_prop : forall f, noccur f prop.
-red; simpl; reflexivity.
-Qed.
-
-  Lemma noc_app : forall f a b,
-    noccur f a -> noccur f b -> noccur f (App a b).
-unfold noccur; simpl; intros.
-rewrite (H _ _ H1).
-rewrite (H0 _ _ H1).
-reflexivity.
-Qed.
-
-
-(********************************************************************************)
-(** Judgements with variance *)
-
-Module Beq.
-Definition t := bool.
-Definition eq := @eq bool.
-Definition eq_equiv : Equivalence eq := eq_equivalence.
-Existing Instance eq_equiv.
-End Beq.
-Module B := VarMap.Make(Beq).
-
-Module OTeq.
-Definition t := option trm.
-Definition eq := @eq (option trm).
-Definition eq_equiv : Equivalence eq := eq_equivalence.
-Existing Instance eq_equiv.
-End OTeq.
-Module OT := VarMap.Make(OTeq).
-
-(* Environments with tags on ordinal and recursive function variables *)
-Record fenv := {
-  tenv : env;
-  ords : B.map; (* variables denoting ordinals *)
-  fixs : OT.map (* variables denoting recursive functions with their domain *)
-}.
-
-Definition tinj e :=
-  Build_fenv e (B.nil false) (OT.nil None).
-
-Definition push_var e T :=
-  Build_fenv (T::tenv e) (B.cons false (ords e)) (OT.cons None (fixs e)).
-
-Definition push_fun e dom rng :=
-  Build_fenv (Prod dom rng::tenv e)
-    (B.cons false (ords e)) (OT.cons (Some dom) (fixs e)).
-
-Definition push_ord e T :=
-  Build_fenv (T::tenv e) (B.cons true (ords e)) (OT.cons None (fixs e)).
-
-
-(* Additional judgments for fix body *)
-Definition val_mono (e:fenv) i j i' j' :=
-    val_ok (tenv e) i j /\
-    val_ok (tenv e) i' j' /\
-    forall n,
-    if ords e n then i n ⊆ i' n
-    else match fixs e n with
-      Some T => forall x, x ∈ El(int T (V.shift (S n) i)) -> app (i n) x == app (i' n) x
-    | _ => i n == i' n
-    end.
-
-Lemma val_mono_refl : forall e i j,
-  val_ok (tenv e) i j -> val_mono e i j i j.
-split;[idtac|split]; simpl; auto with *.
-intro n.
-destruct (ords e n); auto with *.
-destruct (fixs e n); auto with *.
-Qed.
-
-Lemma val_push_var : forall e i j i' j' x t x' t' T,
-  val_mono e i j i' j' ->
-  x == x' ->
-  [x,t] \real int T i ->
-  [x',t'] \real int T i' ->
-  T <> kind ->
-  val_mono (push_var e T) (V.cons x i) (I.cons t j) (V.cons x' i') (I.cons t' j').
-destruct 1 as (?&?&?); split;[idtac|split]; trivial.
- unfold push_var; simpl.
- apply vcons_add_var; trivial.
-
- unfold push_var; simpl.
- apply vcons_add_var; trivial.
-
- destruct n as [|n]; simpl; auto.
- generalize (H1 n).
- destruct (ords e n); trivial.
-Qed.
-
-Lemma val_push_ord : forall e i j i' j' x t x' t' T,
-  val_mono e i j i' j' ->
-  x ⊆ x' ->
-  [x,t] \real int T i ->
-  [x',t'] \real int T i' ->
-  T <> kind ->
-  val_mono (push_ord e T) (V.cons x i) (I.cons t j) (V.cons x' i') (I.cons t' j').
-destruct 1 as (?&?&?); split;[idtac|split]; trivial.
- unfold push_ord; simpl.
- apply vcons_add_var; trivial.
-
- unfold push_ord; simpl.
- apply vcons_add_var; trivial.
-
- destruct n as [|n]; simpl; auto.
- generalize (H1 n).
- destruct (ords e n); trivial.
-Qed.
-
-
-Lemma val_push_fun : forall e i j i' j' f tf g tg T U,
-  val_mono e i j i' j' ->
-  [f,tf] \real int (Prod T U) i ->
-  [g,tg] \real int (Prod T U) i' ->
-  fcompat (El(int T i)) f g ->
-  val_mono (push_fun e T U) (V.cons f i) (I.cons tf j) (V.cons g i') (I.cons tg j').
-destruct 1 as (?&?&?); split;[idtac|split]; trivial.
- unfold push_fun; simpl.
- apply vcons_add_var; trivial.
- discriminate.
-
- unfold push_fun; simpl.
- apply vcons_add_var; trivial.
- discriminate.
-
- destruct n as [|n]; simpl; auto.
- generalize (H1 n).
- destruct (ords e n); trivial.
-Qed.
-
-(** Function Extension judgment *)
-Definition fx_extends e dom M :=
-  forall i i' j j', val_mono e i j i' j' ->
-  fcompat (El(int dom i)) (int M i) (int M i').
-
-(** Covariance judgment *)
-Definition fx_sub e M :=
-  forall i i' j j', val_mono e i j i' j' ->
-  forall x t, [x,t] \real int M i -> [x,t] \real int M i'.
-
-Definition fx_subval e M :=
-  forall i i' j j', val_mono e i j i' j' -> int M i ⊆ int M i'.
-
-(** Invariance *)
-Definition fx_equals e M :=
-  forall i i' j j', val_mono e i j i' j' -> int M i == int M i'.
-
-
-Lemma El_sub e T i j i' j':
-  fx_sub e T ->
-  val_mono e i j i' j' ->
-  El (int T i) ⊆ El (int T i').
-intros.
-apply H in H0.
-red; intros.
-apply H0 with daimon.
-split;[trivial|apply varSAT].
-Qed.
-Lemma El_eq e T i j i' j':
-  fx_equals e T ->
-  val_mono e i j i' j' ->
-  El (int T i) == El (int T i').
-intros.
-apply H in H0.
-rewrite H0; reflexivity.
-Qed.
-
-Require Import Bool.
-
-Definition spec_var e n :=
-  ords e n || match fixs e n with Some _ => true | _ => false end.
-
-  Lemma fx_eq_noc : forall e t,
-    noccur (spec_var e) t ->
-    fx_equals e t.
-unfold noccur, fx_equals, spec_var; intros.
-apply H; intros.
-destruct H0 as (_,(_,H0)).
-generalize (H0 n).
-destruct (ords e n); simpl; trivial.
-destruct (fixs e n); simpl; trivial.
-Qed.
-
-  Lemma fx_eq_app : forall e u v,
-    fx_equals e u ->
-    fx_equals e v ->
-    fx_equals e (App u v).
-unfold fx_equals; intros.
-specialize H with (1:=H1).
-specialize H0 with (1:=H1).
-simpl.
-rewrite H; rewrite H0; reflexivity.
-Qed.
-
-  Lemma fx_eq_abs : forall e T M,
-    T <> kind ->
-    fx_equals e T ->
-    fx_equals (push_var e T) M ->
-    fx_equals e (Abs T M).
-unfold fx_equals; intros.
-simpl.
-apply lam_ext; eauto.
-red; intros.
-apply H1 with (I.cons daimon j) (I.cons daimon j').
-specialize H0 with (1:=H2).
-apply val_push_var; auto.
- split; trivial.
- apply varSAT.
-
- split.
- 2:apply varSAT.
- unfold inX; rewrite <- H4; rewrite <- H0; trivial.
-Qed.
-
-  Lemma fx_eq_rec_call : forall e n x T U,
-    ords e n = false ->
-    fixs e n = Some T ->
-    T <> kind ->
-    typ (tenv e) (Ref n) (Prod (lift (S n) T) U) ->
-    fx_equals e x ->
-    typ (tenv e) x (lift (S n) T) ->
-    fx_equals e (App (Ref n) x).
-unfold fx_equals; intros.
-simpl.
-specialize H3 with (1:=H5).
-rewrite <- H3.
-destruct H5 as (Hty,(Hty',Hrec)).
-specialize Hrec with n.
-rewrite H in Hrec; rewrite H0 in Hrec.
-apply Hrec.
-red in H4; specialize H4 with (1:=Hty); trivial.
-apply in_int_not_kind in H4; trivial.
-2:destruct T;[discriminate|elim H1;reflexivity].
-destruct H4 as (?,_ ).
-unfold inX in H4.
-unfold lift in H4; rewrite int_lift_rec_eq in H4.
-rewrite V.lams0 in H4; trivial.
-Qed.
-
-  (* Covariance *)
-
-  Lemma fx_equals_subval : forall e M, fx_equals e M -> fx_subval e M.
-unfold fx_subval, fx_equals; intros.
-apply H in H0.
-rewrite <- H0; reflexivity.
-Qed.
-
-  Lemma fx_equals_sub : forall e M, fx_equals e M -> fx_sub e M.
-unfold fx_sub, fx_equals; intros.
-apply H in H0.
-destruct H1.
-split.
- red.
- rewrite <- H0; trivial.
-
- rewrite <- H0; trivial.
-Qed.
-
-  Lemma var_sub : forall e n,
-    ords e n = true ->
-    fx_subval e (Ref n).
-unfold fx_subval; intros.
-destruct H0 as (_,(_,H0)).
-generalize (H0 n); rewrite H.
-simpl; trivial.
-Qed.
-
-Lemma fx_sub_prod : forall e T U,
-  T <> kind ->
-  fx_equals e T ->
-  fx_sub (push_var e T) U ->
-  fx_sub e (Prod T U).
-red; intros.
-red in H0; specialize H0 with (1:=H2).
-destruct H3.
-red in H3.
-rewrite El_int_prod in H3.
-rewrite Real_int_prod in H4; trivial.
-apply and_split; intros.
- red; rewrite El_int_prod.
- revert H3; apply cc_prod_covariant; intros.
-  do 2 red; intros.
-  rewrite H5; reflexivity.
-
-  rewrite H0; reflexivity.
-
-  apply El_sub with (1:=H1) (j:=I.cons daimon j) (j':=I.cons daimon j').
-  apply val_push_var; auto with *.
-   split;[trivial|apply varSAT].
-   split;[|apply varSAT].
-   red; rewrite <- H0; trivial.
-
- red in H5; rewrite El_int_prod in H5.
- rewrite Real_int_prod; trivial.
- apply interSAT_intro' with
-   (F:=fun v => prodSAT(Real(int T i') v)(Real(int U (V.cons v i'))(cc_app x v))).
-  apply sat_sn in H4; trivial.
- intros.
- rewrite <- H0 in H6.
- specialize interSAT_elim with (1:=H4) (x:=exist (fun x=> x ∈ El(int T i)) x0 H6); simpl proj1_sig; intros.
- revert H7; apply prodSAT_mono.
-  do 2 red; intros.
-  rewrite <- H0 in H7; trivial.
-
-  red; intros.
-  apply H1 with (i:=V.cons x0 i) (j:=I.cons daimon j) (j':=I.cons daimon j').
-   apply val_push_var; auto with *.
-   split; trivial; apply varSAT.
-   split.
-    red; rewrite <- H0; trivial.
-    apply varSAT.
-
-   split; trivial.
-   unfold inX; apply cc_prod_elim with (1:=H3); trivial.
-Qed.
-
-
-  Lemma Wi_sub : forall e o A B O,
-    isOrd o ->
-    zero ∈ o ->
-    A <> kind ->
-    typ (tenv e) O (Ordt o) ->
-    fx_equals e A ->
-    fx_equals (push_var e A) B ->
-    fx_subval e O ->
-    fx_sub e (WI A B O).
-unfold fx_sub, fx_subval.
-intros e o A B O oo oz Ank tyO eqA eqB subO i i' j j' val_m x t (xreal,xsat).
-destruct tyord_inv with (3:=tyO) (4:=proj1 val_m); trivial.
-destruct tyord_inv with (3:=tyO) (4:=proj1 (proj2 val_m)); trivial.
-red in eqA; specialize eqA with (1:=val_m).
-specialize subO with (1:=val_m).
-red in xreal; rewrite El_int_W in xreal.
-rewrite Real_int_W in xsat; trivial.
-assert (cc_bot (TI (WF' A B i) (int O i)) ⊆ cc_bot (TI (WF' A B i') (int O i'))).
- apply cc_bot_mono.
- transitivity (TI (WF' A B i') (int O i)).
-  intro; apply eq_elim.
-  apply TI_morph_gen; auto with *.
-  red; intros.
-  apply W_F_ext; auto with *.
-   apply El_morph; trivial.
-
-   red; intros.
-   apply El_morph.
-   apply eqB with (I.cons daimon j) (I.cons daimon j').
-    apply val_push_var; auto with *.
-    split; [trivial|apply varSAT].
-    rewrite H5 in H4.
-    rewrite eqA in H4.
-    split; [trivial|apply varSAT].
-
-   apply cc_bot_morph; trivial.
-
-  destruct H0; destruct H2.
-  apply TI_mono; trivial.
-  do 2 red; intros; apply W_F_mono.
-   do 2 red; intros.
-   rewrite H6; reflexivity.
-
-   apply cc_bot_mono; auto with *.
-split.
- red; rewrite El_int_W; auto.
-
- rewrite Real_int_W; auto.
- rewrite cc_bot_ax in xreal; destruct xreal as [H4|xreal].
-  assert (eqSAT (RW A B i (int O i) x) (RW A B i (int O i) empty)).
-   unfold RW; apply rWi_morph; auto with *.
-   do 2 red; intros.
-   rewrite H5; reflexivity.
- rewrite H5 in xsat.
- revert xsat; unfold RW; apply rWi_neutral; trivial.
-  apply Bw_morph; reflexivity.
-  apply RAw_morph; reflexivity.
-
- setoid_replace (RW A B i' (int O i') x) with (RW A B i (int O i) x); trivial.
- symmetry; transitivity (RW A B i (int O i') x).
-  unfold RW; apply rWi_mono; trivial.
-   apply Bw_morph; reflexivity.
-   apply RAw_morph; reflexivity.
-
-  unfold RW; apply rWi_ext; trivial; intros.
-   do 2 red; intros.
-   rewrite H4; reflexivity.
-
-   apply El_morph; trivial.
-
-   red; intros.
-   eapply El_eq with (1:=eqB).
-   apply val_push_var; eauto.
-    split;[trivial|apply varSAT].
-    split;[rewrite eqA in H4;rewrite H5 in H4;trivial|apply varSAT].
- 
-   do 2 red; intros.
-   rewrite eqA; rewrite H4; reflexivity.
-
-   do 2 red; intros.
-   apply Real_morph; trivial.
-   eapply eqB.
-   apply val_push_var; eauto.
-    split;[trivial|apply varSAT].
-    split;[rewrite eqA in H4;rewrite H5 in H4;trivial|apply varSAT].
-
-  reflexivity.
-  reflexivity.
-Qed.
-
-  Lemma OSucc_sub : forall e O,
-    fx_subval e O ->
-    fx_subval e (OSucc O).
-unfold fx_subval; simpl; intros.
-unfold osucc.
-red; intros.
-rewrite subset_ax in H1 |-*.
-destruct H1; split; auto.
-revert H1; apply power_mono.
-eauto.
-Qed.
-
-  (* Function subtyping *)
-
-  Lemma fx_abs : forall e U T M,
-    T <> kind ->
-    fx_sub e T ->
-    fx_equals (push_var e T) M ->
-    typ (T::tenv e) M U ->
-    U <> kind ->
-    fx_extends e T (Abs T M).
-unfold fx_equals, fx_extends; intros.
-specialize El_sub with (1:=H0)(2:=H4); clear H0; intro H0.
-simpl.
-red; intros.
-rewrite beta_eq; try assumption.
- assert (H5' := H0 _ H5).
- rewrite beta_eq; trivial.
-  apply H1 with (I.cons daimon j) (I.cons daimon j').
-  apply val_push_var; auto with *.
-   split; [trivial|apply varSAT].
-
-   split; [trivial|apply varSAT].
-
-  red; red; intros.
-  rewrite H7; reflexivity.
-
- red; red; intros.
- rewrite H7; reflexivity.
-Qed.
 
 (*****************************************************************************)
 (** Recursor (without case analysis) *)
@@ -1088,8 +640,6 @@ exists (fun i =>
 Defined.
 
 
-
-
 (** Typing rules of WFix *)
 
 Section WFixRules.
@@ -1116,14 +666,6 @@ Section WFixRules.
     (WIL 2 (OSucc (Ref 1)))
     M.
 
-  Lemma WF'mono i : Proper (incl_set==>incl_set) (WF' A B i).
-do 2 red; intros.
-unfold WF'.
-apply W_F_mono.
- do 2 red; intros; apply Bw_morph; auto with *.
- apply cc_bot_mono; trivial.
-Qed.
-  Hint Resolve WF'mono.
 
   Let Wi i o := cc_bot (TI (WF' A B i) o).
   Let F i := fun o' f => squash (int M (V.cons f (V.cons o' i))).
@@ -1829,18 +1371,6 @@ apply and_split; intros.
 Qed.
 
 
-Lemma TI_inv i o x :
-  isOrd o ->
-  x ∈ TI (WF' A B i) o ->
-  exists2 o', o' ∈ o & x ∈ TI (WF' A B i) (osucc o').
-intros.
-apply TI_elim in H0; auto.
-destruct H0.
-exists x0; trivial.
-rewrite TI_mono_succ; trivial.
-apply isOrd_inv with o; trivial.
-Qed.
-
 (** Fixpoint equation holds only when applied to a constructor,
     because of the realizability part of the interpretation.
  *)
@@ -2068,94 +1598,94 @@ change e with (tenv (tinj e)).
 apply typ_wfix with (infty:=infty); trivial.
 Qed.
 
-(****************************************************************************************)
-(** Compound judgements : typing + variance *)
 
-Definition typ_ext e M A B :=
-  fx_extends e A M /\ typ (tenv e) M (Prod A B).
+(** Variance results *)
 
-Definition typ_mono e M :=
-  fx_sub e M /\ typs (tenv e) M.
+  Lemma Wi_sub : forall e o A B O,
+    isOrd o ->
+    zero ∈ o ->
+    A <> kind ->
+    typ (tenv e) O (Ordt o) ->
+    fx_equals e A ->
+    fx_equals (push_var e A) B ->
+    fx_subval e O ->
+    fx_sub e (WI A B O).
+unfold fx_sub, fx_subval.
+intros e o A B O oo oz Ank tyO eqA eqB subO i i' j j' val_m x t (xreal,xsat).
+destruct tyord_inv with (3:=tyO) (4:=proj1 val_m); trivial.
+destruct tyord_inv with (3:=tyO) (4:=proj1 (proj2 val_m)); trivial.
+red in eqA; specialize eqA with (1:=val_m).
+specialize subO with (1:=val_m).
+red in xreal; rewrite El_int_W in xreal.
+rewrite Real_int_W in xsat; trivial.
+assert (cc_bot (TI (WF' A B i) (int O i)) ⊆ cc_bot (TI (WF' A B i') (int O i'))).
+ apply cc_bot_mono.
+ transitivity (TI (WF' A B i') (int O i)).
+  intro; apply eq_elim.
+  apply TI_morph_gen; auto with *.
+  red; intros.
+  apply W_F_ext; auto with *.
+   apply El_morph; trivial.
 
-Definition typ_monoval e M T :=
-  fx_subval e M /\ typ (tenv e) M T.
+   red; intros.
+   apply El_morph.
+   apply eqB with (I.cons daimon j) (I.cons daimon j').
+    apply val_push_var; auto with *.
+    split; [trivial|apply varSAT].
+    rewrite H5 in H4.
+    rewrite eqA in H4.
+    split; [trivial|apply varSAT].
 
-Definition typ_impl e M T :=
-  fx_equals e M /\ typ (tenv e) M T.
+   apply cc_bot_morph; trivial.
 
-Instance typ_impl_morph e : Proper (eq_trm ==> eq_trm ==> iff) (typ_impl e).
-apply morph_impl_iff2; auto with *.
-do 4 red; intros.
-destruct H1; split.
- red; intros.
- rewrite <- H; eauto.
-
- rewrite <- H; rewrite <- H0; eauto.
-Qed.
-
-Lemma typ_var_impl : forall e n t T,
-    spec_var e n = false ->
-    nth_error (tenv e) n = value t ->
-    t <> kind ->
-    T <> kind ->
-    sub_typ (tenv e) (lift (S n) t) T ->
-    typ_impl e (Ref n) T.
-intros.
+  destruct H0; destruct H2.
+  apply TI_mono; trivial.
 split.
- apply fx_eq_noc; apply noc_var; trivial.
+ red; rewrite El_int_W; auto.
 
- apply typ_subsumption with (lift (S n) t); trivial.
-  apply typ_var; trivial.
+ rewrite Real_int_W; auto.
+ rewrite cc_bot_ax in xreal; destruct xreal as [H4|xreal].
+  assert (eqSAT (RW A B i (int O i) x) (RW A B i (int O i) empty)).
+   unfold RW; apply rWi_morph; auto with *.
+   do 2 red; intros.
+   rewrite H5; reflexivity.
+ rewrite H5 in xsat.
+ revert xsat; unfold RW; apply rWi_neutral; trivial.
+  apply Bw_morph; reflexivity.
+  apply RAw_morph; reflexivity.
 
-  destruct t as [(t,tm)|]; simpl in *; auto.
-  discriminate.
-Qed.
+ setoid_replace (RW A B i' (int O i') x) with (RW A B i (int O i) x); trivial.
+ symmetry; transitivity (RW A B i (int O i') x).
+  unfold RW; apply rWi_mono; trivial.
+   apply Bw_morph; reflexivity.
+   apply RAw_morph; reflexivity.
 
-  Lemma impl_abs : forall e s1 U T T' M,
-    T <> kind ->
-    U <> kind ->
-    s1=prop \/ s1=kind ->
-    eq_typ (tenv e) T T' ->
-    typ_impl e T s1 ->
-    typ_impl (push_var e T) M U ->
-    typ_impl e (Abs T M) (Prod T' U).
-intros.
-destruct H3; destruct H4.
-split.
- apply fx_eq_abs; trivial.
+  unfold RW; apply rWi_ext; trivial; intros.
+   do 2 red; intros.
+   rewrite H4; reflexivity.
 
- apply typ_conv with (Prod T U); auto.
-  apply typ_abs; trivial.
-  destruct H1; subst s1; red; auto.
+   apply El_morph; trivial.
 
-  apply eq_typ_prod; trivial.
+   red; intros.
+   eapply El_eq with (1:=eqB).
+   apply val_push_var; eauto.
+    split;[trivial|apply varSAT].
+    split;[rewrite eqA in H4;rewrite H5 in H4;trivial|apply varSAT].
+ 
+   do 2 red; intros.
+   rewrite eqA; rewrite H4; reflexivity.
+
+   do 2 red; intros.
+   apply Real_morph; trivial.
+   eapply eqB.
+   apply val_push_var; eauto.
+    split;[trivial|apply varSAT].
+    split;[rewrite eqA in H4;rewrite H5 in H4;trivial|apply varSAT].
+
   reflexivity.
-
-  discriminate.
-
-  discriminate.
+  reflexivity.
 Qed.
 
-Lemma impl_app : forall e u v V Ur T,
-  T <> kind ->
-  V <> kind ->
-  Ur <> kind ->
-  sub_typ (tenv e) (subst v Ur) T ->
-  typ_impl e u (Prod V Ur) ->
-  typ_impl e v V ->
-  typ_impl e (App u v) T.
-intros.
-destruct H3.
-destruct H4.
-split.
- apply fx_eq_app; trivial.
-
- apply typ_subsumption with (subst v Ur); trivial.
-  apply typ_app with V; auto.
-
-  destruct Ur as [(Ur,Urm)|]; simpl; trivial.
-  discriminate.
-Qed.
 
   Lemma Wi_fx_sub : forall e o A B O,
     isOrd o ->
@@ -2175,98 +1705,6 @@ revert i i' j j' H4 x t H5.
 change (fx_sub e (WI A B O)).
 apply Wi_sub with (o:=o); trivial.
 Qed.
-
-  Lemma OSucc_fx_sub : forall e O o,
-    isOrd o ->
-    zero ∈ o ->
-    typ_monoval e O (Ordt o)->
-    typ_monoval e (OSucc O) (Ordt (osucc o)).
-destruct 3.
-split.
- apply OSucc_sub; trivial.
-
- red; simpl; intros.
- apply in_int_intro; try discriminate.
- destruct tyord_inv with (3:=H2)(4:=H3) as (_,(?,_)); trivial.
- assert (osucc (int O i) ∈ El (int (Ordt (osucc o)) i)).
-  rewrite El_int_ord.
-  apply lt_osucc_compat; trivial.
-  apply ole_lts; auto.
- split; simpl; trivial.
- rewrite Real_def; auto with *.
-  assert (h:= H2 _ _ H3).
-  apply in_int_sn in h.
-  simpl; trivial.
-
-  simpl.
-  apply cc_bot_intro.
-  apply lt_osucc_compat; trivial.
-Qed.
-
-  Lemma typ_var_mono : forall e n t T,
-    ords e n = true ->
-    nth_error (tenv e) n = value t ->
-    T <> kind ->
-    t <> kind ->
-    sub_typ (tenv e) (lift (S n) t) T ->
-    typ_monoval e (Ref n) T.
-intros.
-split.
- apply var_sub; trivial.
-
- apply typ_subsumption with (lift (S n) t); trivial.
-  apply typ_var; trivial.
-
-  destruct t as [(t,tm)|]; simpl in *; auto.
-  discriminate.
-Qed.
-
-  Lemma ext_abs : forall e U T M,
-    T <> kind ->
-    U <> kind ->
-    typ_mono e T ->
-    typ_impl (push_var e T) M U ->
-    typ_ext e (Abs T M) T U.
-intros.
-destruct H1; destruct H2; split.
- apply fx_abs with U; trivial.
-
- apply typ_abs; trivial.
-Qed.
-
-(*************)
-
-  Lemma impl_call : forall e n x t u T,
-    ords e n = false ->
-    fixs e n = Some t ->
-    T <> kind ->
-    t <> kind ->
-    u <> kind ->
-    nth_error (tenv e) n = value (Prod t u) ->
-    sub_typ (tenv e) (subst x (lift_rec (S n) 1 u)) T ->
-    typ_impl e x (lift (S n) t) ->
-    typ_impl e (App (Ref n) x) T.
-intros.
-destruct H6.
-assert (typ (tenv e) (Ref n) (Prod (lift (S n) t) (lift_rec (S n) 1 u))).
- apply typ_var0; rewrite H4; split;[discriminate|].
- apply sub_refl.
-
- unfold lift; rewrite red_lift_prod.
- reflexivity.
-split.
- apply fx_eq_rec_call with t (lift_rec (S n) 1 u); trivial.
-
- apply typ_subsumption with (subst x (lift_rec (S n) 1 u)); auto.
- 2:destruct u as [(u,um)|]; trivial.
- 2:discriminate.
- apply typ_app with (lift (S n) t); trivial.
- destruct t as [(t,tm)|]; trivial.
- discriminate.
- destruct u as [(u,um)|]; trivial.
- discriminate.
-Qed.
-
 
 Lemma typ_wfix'' : forall infty e A B O U M T,
        isOrd infty ->
