ZFecc.v
@@ -1,8 +1,98 @@
 Require Import ZF ZFpairs ZFnats ZFgrothendieck.
 Require Import ZFrelations ZFcoc.
 
+(** Statement that there exists a set containing infinitely many Grothendieck universes *)
+
+(*Definition infinitely_many_universes :=
+  { U:set | empty ∈ U /\ forall x, x ∈ U -> grot_succ x ∈ U }.*)
+Definition infinitely_many_universes :=
+  { U:set | empty ∈ U /\ forall x, x ∈ U -> exists V, V ∈ U /\ grot_univ V /\ x ∈ V }.
+(*
+Instance grot_succ_pred_mono : Proper (eq_set==>eq_set==>iff) grot_succ_pred.
+do 3 red; intros.
+apply and_iff_morphism.
+ split; apply grot_univ_ext; auto with *.
+apply and_iff_morphism.
+ apply in_set_morph; trivial.
+apply fa_morph; intros U.
+rewrite H; rewrite H0; reflexivity.
+Qed.
+*)
+
+Instance grot_succ_pred_morph : Proper (eq_set==>eq_set==>iff) grot_succ_pred.
+do 3 red; intros.
+apply and_iff_morphism.
+ split; apply grot_univ_ext; auto with *.
+apply and_iff_morphism.
+ apply in_set_morph; trivial.
+apply fa_morph; intros U.
+rewrite H; rewrite H0; reflexivity.
+Qed.
+
+Lemma grot_succ_incl x y :
+  x ∈ grot_succ y ->
+  ZFrepl.uchoice_pred (grot_succ_pred x) ->
+  ZFrepl.uchoice_pred (grot_succ_pred y) ->
+  grot_succ x ⊆ grot_succ y.
+intros.
+specialize ZFrepl.uchoice_def with (1:=H0); intros (?,(?,xmin)).
+specialize ZFrepl.uchoice_def with (1:=H1); intros (?,(?,_)).
+apply xmin; trivial.
+Qed.
+Lemma grot_succ_mono x y :
+  x ⊆ y ->
+  ZFrepl.uchoice_pred (grot_succ_pred x) ->
+  ZFrepl.uchoice_pred (grot_succ_pred y) ->
+  grot_succ x ⊆ grot_succ y.
+intros.
+apply grot_succ_incl; trivial.
+specialize ZFrepl.uchoice_def with (1:=H1); intros (?,(?,_)).
+apply G_incl with y; trivial.
+Qed.
+
+(** In Tarski-Grothendieck set theory, there exists an infinite sequence of universes *)
+Lemma tg_implies_ecc : grothendieck -> infinitely_many_universes.
+assert (gsm : morph1 grot_succ).
+ do 2 red ;intros.
+ apply ZFrepl.uchoice_morph_raw.
+ red; intros.
+ apply grot_succ_pred_morph; trivial.
+intros gr.
+exists (ZFord.TI grot_succ ZFord.omega).
+split; intros.
+ apply ZFord.TI_intro with (ZFord.osucc zero); auto.
+ eapply G_incl.
+  apply (grot_succ_typ gr).
+
+  apply (grot_succ_in gr).
+
+  red; intros.
+  apply empty_ax in H; contradiction.
+
+ apply ZFord.TI_elim in H; auto.
+ destruct H as (o,?,?).
+ assert (oo: ZFord.isOrd o) by eauto using ZFord.isOrd_inv.
+ exists (grot_succ (ZFord.TI grot_succ o)).
+ split;[|split]; trivial.
+ 2:apply (grot_succ_typ gr).
+ apply ZFord.TI_intro with (ZFord.osucc o); auto.
+ eapply G_incl.
+  apply (grot_succ_typ gr).
+
+  apply (grot_succ_in gr).
+
+  red; intros.
+  apply ZFord.TI_intro with o; auto.
+Qed.
+
+(*
 (* We are in Tarski-Grothendieck set theory: *)
 Axiom gr : grothendieck.
+*)
+
+Axiom infinite_seq_of_grot_univ : infinitely_many_universes.
+
+Let U := proj1_sig infinite_seq_of_grot_univ.
 
 Fixpoint ecc (n:nat) : set :=
   match n with
@@ -10,29 +100,134 @@ Fixpoint ecc (n:nat) : set :=
   | S k => grot_succ (ecc k)
   end.
 
+Lemma grot_succU y x :
+  y ⊆ x -> 
+  x ∈ U ->
+  grot_univ (grot_succ y) /\ y ∈ grot_succ y /\ exists2 W, W ∈ U & grot_succ y ⊆ W.
+intros.
+destruct (proj2_sig infinite_seq_of_grot_univ) as (_,nextU); fold U in *.
+destruct nextU with (1:=H0) as (V,(VU,(gV,xV))).
+pose (W:=subset V (fun z =>
+    forall U, grot_univ U -> y ∈ U -> z ∈ U)).
+assert (grot_succ_pred y W).
+ split;[|split]; intros.
+  apply grot_intersection; trivial.
+  apply G_incl with x; auto.
+
+  apply subset_intro; trivial.
+  apply G_incl with x; auto.
+
+  red; intros.
+  unfold W in H3; rewrite subset_ax in H3; destruct H3.
+  destruct H4 as (z',eqz,min).
+  rewrite eqz; auto.
+assert (ZFrepl.uchoice_pred (grot_succ_pred y)).
+ split;[|split]; intros.
+  revert H3; apply grot_succ_pred_morph; auto with *.
+
+  exists W; trivial.
+
+  destruct H2 as (?,(?,?)).
+  destruct H3 as (?,(?,?)).
+  apply incl_eq; auto.
+specialize ZFrepl.uchoice_ext with (1:=H2)(2:=H1); intro.
+fold (grot_succ y) in H3.
+split.
+ apply grot_univ_ext with W; auto.
+ apply H1.
+split.
+ destruct H1 as (_,(?,_)).
+ rewrite <- H3; trivial.
+
+ exists V; trivial.
+ rewrite <- H3.
+ red; intros.
+ apply subset_elim1 in H4; trivial.
+Qed.
+
+
+Lemma grot_succ_hf : grot_succ empty == grot_succ props.
+  apply ZFrepl.uchoice_morph_raw.
+  red; intros.
+  unfold grot_succ_pred.
+  split; intros.
+   destruct H0.
+   assert (grot_univ y).
+    revert H0; apply grot_univ_ext; auto.
+   split; trivial.
+   destruct H1; split; intros.
+    apply G_power; trivial.
+    apply G_singl; trivial.
+    rewrite <- H; trivial.
+
+    rewrite <- H; apply H3; trivial.
+    apply G_incl with props; trivial.
+    red; intros.
+    apply empty_ax in H6; contradiction.
+
+   destruct H0.
+   assert (grot_univ x).
+    revert H0; apply grot_univ_ext; auto with *.
+   split; trivial.
+   destruct H1; split; intros.
+    rewrite H.
+    apply G_incl with props; trivial.
+    red; intros.
+    apply empty_ax in H4; contradiction.
+
+    rewrite H; apply H3; trivial.
+    apply G_power; trivial.
+    apply G_singl; trivial.
+Qed.
+
+Lemma ecc_U : forall n, grot_univ (ecc n) /\ exists2 W, W ∈ U & ecc n ⊆ W.
+destruct (proj2_sig infinite_seq_of_grot_univ) as (mtU, nextU); fold U in *.
+induction n; simpl; intros.
+ destruct grot_succU with empty empty as (?,(_,?)); auto with *.
+ split; intros.
+  revert H; apply grot_univ_ext; auto with *.
+  apply grot_succ_hf.
+
+  destruct H0.
+  exists x; trivial.
+  rewrite <- grot_succ_hf; trivial.
+
+ destruct IHn as (?,(W,?,?)).
+ destruct grot_succU with (1:=H1)(2:=H0) as (?,(_,?)); auto.
+Qed.
+
 Lemma ecc_grot : forall n, grot_univ (ecc n).
-destruct n; apply (grot_succ_typ gr).
+intros.
+apply ecc_U.
 Qed.
 Hint Resolve ecc_grot.
 
-Lemma ecc_in1 : forall n, props ∈ ecc n.
-induction n; simpl; intros.
- apply (grot_succ_in gr).
- apply G_trans with (ecc n); trivial.
-  apply (grot_succ_typ gr).
-
-  apply (grot_succ_in gr).
-Qed.
-
 Lemma ecc_in2 : forall n, ecc n ∈ ecc (S n).
 simpl; intros.
-apply (grot_succ_in gr).
+destruct ecc_U with n as (?,(W,?,?)).
+destruct grot_succU with (1:=H1)(2:=H0) as (_,(?,_)); trivial.
 Qed.
+
+Lemma ecc_in1 : forall n, props ∈ ecc n.
+induction n; simpl; intros.
+ destruct grot_succU with empty empty as (?,(?,?)); auto with *.
+  apply (proj2_sig infinite_seq_of_grot_univ).
+
+  rewrite <- grot_succ_hf.
+  apply G_power; trivial.
+  apply G_singl; trivial.
+
+ apply G_trans with (ecc n); trivial.
+  apply (ecc_grot (S n)).
+
+  apply ecc_in2.
+Qed.
+ 
 
 Lemma ecc_incl : forall n x, x ∈ ecc n -> x ∈ ecc (S n).
 simpl; intros.
 apply G_trans with (ecc n); trivial.
- apply (grot_succ_typ gr).
+ apply (ecc_grot (S n)).
 
  apply ecc_in2.
 Qed.
@@ -46,10 +241,9 @@ Qed.
 Lemma ecc_incl_prop : forall x, x ∈ props -> x ∈ ecc 0.
 simpl; intros.
 apply G_trans with props; trivial.
- apply (grot_succ_typ gr).
+ apply (ecc_grot 0).
 
- apply grot_succ_in.
- exact gr.
+ apply (ecc_in1 0).
 Qed.
 
 Lemma ecc_prod : forall n X Y,
@@ -139,7 +333,7 @@ Qed.
 
 Lemma omega_in_ecc n : ZFord.omega ∈ ecc (S n).
 apply G_incl with (ecc n); auto.
- apply grot_succ_in; exact gr.
+ apply ecc_in2.
 
  apply omega_incl_ecc.
 Qed.
