ModelZF.v
@@ -87,11 +87,61 @@ End CCM.
 
 Module BuildModel := MakeModel(CCM).
 
+Import BuildModel T J R.
+
+Lemma El_int_arr T U i :
+  int (Prod T (lift 1 U)) i == cc_arr (int T i) (int U i).
+simpl.
+apply cc_prod_ext.
+ reflexivity.
+
+ red; intros.
+ rewrite simpl_int_lift.
+ rewrite lift0_term; reflexivity.
+Qed.
+(** Subtyping *)
+
+(*
+Definition sub_typ_covariant : forall e U1 U2 V1 V2,
+  U1 <> kind ->
+  eq_typ e U1 U2 ->
+  sub_typ (U1::e) V1 V2 ->
+  sub_typ e (Prod U1 V1) (Prod U2 V2).
+intros.
+apply sub_typ_covariant; trivial.
+intros.
+unfold eqX, lam, app.
+unfold inX in H2.
+unfold prod, ZFuniv_real.prod in H2; rewrite El_def in H2.
+apply cc_eta_eq in H2; trivial.
+Qed.
+*)
+
+(** Universes *)
+(*
+Lemma cumul_Type : forall e n, sub_typ e (type n) (type (S n)).
+red; simpl; intros.
+red; intros.
+apply ecc_incl; trivial.
+Qed.
+
+Lemma cumul_Prop : forall e, sub_typ e prop (type 0).
+red; simpl; intros.
+red; intros.
+apply G_trans with props; trivial.
+ apply (grot_succ_typ gr).
+
+ apply (grot_succ_in gr).
+Qed.
+*)
+
+
+(** The model in ZF implies the consistency of CC *)
+
 Require Import Term Env.
 Require Import TypeJudge.
 Load "template/Library.v".
 
-(** Consistency of CC *)
 Lemma cc_consistency : forall M M', ~ eq_typ nil M M' FALSE.
 Proof.
 unfold FALSE; red in |- *; intros.
