Model_variance.v
@@ -1,0 +1,575 @@
+Require Import Bool.
+Require Import ZF ZFcoc ZFfunext.
+Require Import ModelZF.
+
+Import BuildModel.
+Import T J R.
+
+(********************************************************************************)
+(** Occurrences *)
+
+Module Beq.
+Definition t := bool.
+Definition eq := @eq bool.
+Definition eq_equiv : Equivalence eq := eq_equivalence.
+Existing Instance eq_equiv.
+End Beq.
+Module B := VarMap.Make(Beq).
+
+
+  (* Non-occurrence : interp do not depend on variables in set [f] *)
+  Definition noccur (f:B.map) (T:term) : Prop :=
+    forall i i',
+    (forall n, if f n then True else i n == i' n) ->
+    int T i == int T i'.
+
+  Lemma noc_var : forall f n, f n = false -> noccur f (Ref n).
+red; simpl; intros.
+specialize (H0 n).
+rewrite H in H0; trivial.
+Qed.
+
+  Lemma noc_cst : forall f x, noccur f (cst x).
+red; simpl; reflexivity.
+Qed.
+
+  Lemma noc_kind : forall f, noccur f kind.
+red; simpl; reflexivity.
+Qed.
+
+  Lemma noc_prop : forall f, noccur f prop.
+intros; apply noc_cst.
+Qed.
+
+  Lemma noc_app : forall f a b,
+    noccur f a -> noccur f b -> noccur f (App a b).
+unfold noccur; simpl; intros.
+rewrite (H _ _ H1).
+rewrite (H0 _ _ H1).
+reflexivity.
+Qed.
+
+  Lemma noc_abs a b f :
+    noccur f a ->
+    noccur (B.cons false f) b ->
+    noccur f (Abs a b).
+red; simpl; intros.
+apply cc_lam_ext.
+ apply H; trivial.
+
+ red; intros.
+ apply H0.
+ destruct n; simpl; trivial.
+ apply H1.
+Qed.
+
+  Lemma noc_prod a b f :
+    noccur f a ->
+    noccur (B.cons false f) b ->
+    noccur f (Prod a b).
+red; simpl; intros.
+apply cc_prod_ext.
+ apply H; trivial.
+
+ red; intros.
+ apply H0.
+ destruct n; simpl; trivial.
+ apply H1.
+Qed.
+
+Ltac noc_tac :=
+  lazymatch goal with 
+    |- noccur _ (App _ _) => apply noc_app; noc_tac
+  | |- noccur _ (Abs _ _) => apply noc_abs; noc_tac
+  | |- noccur _ (Prod _ _) => apply noc_prod; noc_tac
+  | |- noccur _ (Ref _) => apply noc_var; reflexivity
+  | |- noccur _ _ => try (red; reflexivity) (* closed case *)
+  end.
+
+(********************************************************************************)
+(** Judgements with variance *)
+
+Module OTeq.
+Definition t := option term.
+Definition eq := @eq (option term).
+Definition eq_equiv : Equivalence eq := eq_equivalence.
+Existing Instance eq_equiv.
+End OTeq.
+Module OT := VarMap.Make(OTeq).
+
+(* Environments with tags on ordinal and recursive function variables *)
+Record fenv := {
+  tenv : env;
+  ords : B.map; (* variables denoting ordinals *)
+  fixs : OT.map (* variables denoting recursive functions with their domain *)
+}.
+
+Definition tinj e :=
+  Build_fenv e (B.nil false) (OT.nil None).
+
+Definition push_var e T :=
+  Build_fenv (T::tenv e) (B.cons false (ords e)) (OT.cons None (fixs e)).
+
+Definition push_fun e dom rng :=
+  Build_fenv (Prod dom rng::tenv e)
+    (B.cons false (ords e)) (OT.cons (Some dom) (fixs e)).
+
+Definition push_ord e T :=
+  Build_fenv (T::tenv e) (B.cons true (ords e)) (OT.cons None (fixs e)).
+
+
+(* Additional judgments for fix body *)
+Definition val_mono (e:fenv) i i' :=
+    val_ok (tenv e) i /\
+    val_ok (tenv e) i' /\
+    forall n,
+    if ords e n then i n ⊆ i' n
+    else match fixs e n with
+      Some T => forall x, x ∈ int T (V.shift (S n) i) -> cc_app (i n) x == cc_app (i' n) x
+    | _ => i n == i' n
+    end.
+
+Lemma val_mono_refl : forall e i,
+  val_ok (tenv e) i -> val_mono e i i.
+split;[idtac|split]; simpl; auto with *.
+intro n.
+destruct (ords e n); auto with *.
+destruct (fixs e n); auto with *.
+Qed.
+
+Lemma val_push_var : forall e i i' x x' T,
+  val_mono e i i' ->
+  x == x' ->
+  x ∈ int T i ->
+  x' ∈ int T i' ->
+  val_mono (push_var e T) (V.cons x i) (V.cons x' i').
+destruct 1 as (?&?&?); split;[idtac|split]; trivial.
+ unfold push_var; simpl.
+ apply vcons_add_var; trivial.
+
+ unfold push_var; simpl.
+ apply vcons_add_var; trivial.
+
+ destruct n as [|n]; simpl; auto.
+ generalize (H1 n).
+ destruct (ords e n); trivial.
+Qed.
+
+Lemma val_push_ord : forall e i i' x x' T,
+  val_mono e i i' ->
+  x ⊆ x' ->
+  x ∈ int T i ->
+  x' ∈ int T i' ->
+  val_mono (push_ord e T) (V.cons x i) (V.cons x' i').
+destruct 1 as (?&?&?); split;[idtac|split]; trivial.
+ unfold push_ord; simpl.
+ apply vcons_add_var; trivial.
+
+ unfold push_ord; simpl.
+ apply vcons_add_var; trivial.
+
+ destruct n as [|n]; simpl; auto.
+ generalize (H1 n).
+ destruct (ords e n); trivial.
+Qed.
+
+
+Lemma val_push_fun : forall e i i' f g T U,
+  val_mono e i i' ->
+  f ∈ int (Prod T U) i ->
+  g ∈ int (Prod T U) i' ->
+  fcompat (int T i) f g ->
+  val_mono (push_fun e T U) (V.cons f i) (V.cons g i').
+destruct 1 as (?&?&?); split;[idtac|split]; trivial.
+ unfold push_fun; simpl.
+ apply vcons_add_var; trivial.
+
+ unfold push_fun; simpl.
+ apply vcons_add_var; trivial.
+
+ destruct n as [|n]; simpl; auto.
+ generalize (H1 n).
+ destruct (ords e n); trivial.
+Qed.
+
+(** Invariance *)
+Definition var_equals e M :=
+  forall i i', val_mono e i i' -> int M i == int M i'.
+
+(** Covariance judgment *)
+Definition var_mono e M :=
+  forall i i', val_mono e i i' ->
+  int M i ⊆ int M i'.
+
+(** Function Extension judgment *)
+Definition var_ext e dom M :=
+  forall i i', val_mono e i i' ->
+  fcompat (int dom i) (int M i) (int M i').
+
+Lemma El_sub e T i i':
+  var_mono e T ->
+  val_mono e i i' ->
+  int T i ⊆ int T i'.
+intros.
+apply H in H0.
+red; auto.
+Qed.
+Lemma El_eq e T i i':
+  var_equals e T ->
+  val_mono e i i' ->
+  int T i == int T i'.
+intros.
+apply H in H0.
+rewrite H0; reflexivity.
+Qed.
+
+
+Definition spec_var e n :=
+  ords e n || match fixs e n with Some _ => true | _ => false end.
+
+  Lemma var_eq_noc : forall e t,
+    noccur (spec_var e) t ->
+    var_equals e t.
+unfold noccur, var_equals, spec_var; intros.
+apply H; intros.
+destruct H0 as (_,(_,H0)).
+generalize (H0 n).
+destruct (ords e n); simpl; trivial.
+destruct (fixs e n); simpl; trivial.
+Qed.
+
+  Lemma var_eq_app : forall e u v,
+    var_equals e u ->
+    var_equals e v ->
+    var_equals e (App u v).
+unfold var_equals; intros.
+specialize H with (1:=H1).
+specialize H0 with (1:=H1).
+simpl.
+rewrite H; rewrite H0; reflexivity.
+Qed.
+
+  Lemma var_eq_abs : forall e T M,
+    var_equals e T ->
+    var_equals (push_var e T) M ->
+    var_equals e (Abs T M).
+unfold var_equals; intros.
+simpl.
+apply cc_lam_ext; eauto.
+red; intros.
+apply H0.
+specialize H with (1:=H1).
+apply val_push_var; auto.
+rewrite <- H3; rewrite <- H; trivial.
+Qed.
+
+  Lemma var_eq_prod : forall e T U,
+    var_equals e T ->
+    var_equals (push_var e T) U ->
+    var_equals e (Prod T U).
+red; simpl; intros.
+specialize (H _ _ H1).
+apply cc_prod_ext; trivial.
+red; intros.
+apply H0.
+apply val_push_var; auto with *.
+rewrite <- H3.
+rewrite <- H; trivial.
+Qed.
+
+  Lemma var_eq_rec_call : forall e n x T U,
+    ords e n = false ->
+    fixs e n = Some T ->
+    T <> kind ->
+    typ (tenv e) (Ref n) (Prod (lift (S n) T) U) ->
+    var_equals e x ->
+    typ (tenv e) x (lift (S n) T) ->
+    var_equals e (App (Ref n) x).
+unfold var_equals; intros.
+simpl.
+specialize H3 with (1:=H5).
+rewrite <- H3.
+destruct H5 as (Hty,(Hty',Hrec)).
+specialize Hrec with n.
+rewrite H in Hrec; rewrite H0 in Hrec.
+apply Hrec.
+red in H4; specialize H4 with (1:=Hty); trivial.
+apply in_int_not_kind in H4; trivial.
+2:destruct T as [(T,Tm)|];simpl;[discriminate|elim H1;reflexivity].
+unfold lift in H4; rewrite int_lift_rec_eq in H4.
+rewrite V.lams0 in H4; trivial.
+Qed.
+
+  (** Covariance rules *)
+
+  Lemma var_eq_sub : forall e M, var_equals e M -> var_mono e M.
+unfold var_mono, var_equals; intros.
+apply H in H0.
+rewrite <- H0; reflexivity.
+Qed.
+
+  Lemma var_mono_ref : forall e n,
+    ords e n = true ->
+    var_mono e (Ref n).
+unfold var_mono; intros.
+destruct H0 as (_,(_,H0)).
+generalize (H0 n); rewrite H.
+simpl; intros; trivial.
+Qed.
+
+Lemma var_mono_prod : forall e T U,
+  var_equals e T ->
+  var_mono (push_var e T) U ->
+  var_mono e (Prod T U).
+red; red; intros.
+red in H; specialize H with (1:=H1).
+revert H2; simpl; apply cc_prod_covariant; intros.
+ do 2 red; intros.
+ rewrite H3; reflexivity.
+
+ rewrite H; reflexivity.
+
+ apply El_sub with (1:=H0).
+ apply val_push_var; auto with *.
+ rewrite <- H; trivial.
+Qed.
+
+  (** Function subtyping rules *)
+
+  Lemma var_ext_abs : forall e U T M,
+    var_mono e T ->
+    var_equals (push_var e T) M ->
+    typ (T::tenv e) M U ->
+    var_ext e T (Abs T M).
+unfold var_equals, var_ext; intros.
+specialize El_sub with (1:=H)(2:=H2); clear H; intro H.
+simpl.
+red; intros.
+rewrite cc_beta_eq; try assumption.
+ assert (H3' := H _ H3).
+ rewrite cc_beta_eq; trivial.
+  apply H0.
+  apply val_push_var; auto with *.
+
+  red; red; intros.
+  rewrite H5; reflexivity.
+
+ red; red; intros.
+ rewrite H5; reflexivity.
+Qed.
+
+(****************************************************************************************)
+(** Compound judgements : typing + variance *)
+
+Definition typ_equals e M T :=
+  var_equals e M /\ typ (tenv e) M T.
+
+Definition typ_mono e M T :=
+  var_mono e M /\ typ (tenv e) M T.
+
+Definition typ_ext e M A B :=
+  var_ext e A M /\ typ (tenv e) M (Prod A B).
+
+Instance typ_equals_morph e : Proper (eq_term ==> eq_term ==> iff) (typ_equals e).
+apply morph_impl_iff2; auto with *.
+do 4 red; intros.
+destruct H1; split.
+ red; intros.
+ rewrite <- H; eauto.
+
+ rewrite <- H; rewrite <- H0; eauto.
+Qed.
+
+(** ** Inference rules *)
+
+(** Inclusion relation between judgements *)
+
+  Lemma typ_eq_mono : forall e M T, typ_equals e M T -> typ_mono e M T.
+destruct 1; split; trivial.
+apply var_eq_sub; trivial.
+Qed.
+
+  Lemma typ_eq_ext : forall e M A B, typ_equals e M (Prod A B) -> typ_ext e M A B.
+destruct 1; split; trivial.
+do 2 red; intros.
+apply H in H1.
+rewrite H1; reflexivity.
+Qed.
+
+(** Subsumption *)
+  Lemma typ_eq_subsumption e M T T' :
+    typ_equals e M T -> sub_typ (tenv e) T T' -> T <> kind -> typ_equals e M T'.
+destruct 1; split; trivial.
+apply typ_subsumption with (2:=H1); trivial.
+Qed.
+
+(** Typing the three kind of variables *)
+
+  Lemma typ_eq_ref : forall e n T,
+    spec_var e n = false ->
+    nth_error (tenv e) n = value T ->
+    typ_equals e (Ref n) (lift (S n) T).
+intros.
+split.
+ apply var_eq_noc; apply noc_var; trivial.
+ apply typ_var; trivial.
+Qed.
+
+  Lemma typ_mono_ref : forall e n t T,
+    ords e n = true ->
+    nth_error (tenv e) n = value t ->
+    T <> kind ->
+    t <> kind ->
+    sub_typ (tenv e) (lift (S n) t) T ->
+    typ_mono e (Ref n) T.
+intros.
+split.
+ apply var_mono_ref; trivial.
+
+ apply typ_subsumption with (lift (S n) t); trivial.
+  apply typ_var; trivial.
+
+  destruct t as [(t,tm)|]; simpl in *; auto.
+  discriminate.
+Qed.
+
+  Lemma typ_eq_abs : forall e s1 U T T' M,
+    U <> kind ->
+    s1=prop \/ s1=kind ->
+    eq_typ (tenv e) T T' ->
+    typ_equals e T s1 ->
+    typ_equals (push_var e T) M U ->
+    typ_equals e (Abs T M) (Prod T' U).
+intros.
+destruct H2; destruct H3.
+split.
+ apply var_eq_abs; trivial.
+
+ apply typ_conv with (Prod T U); auto.
+  apply typ_abs; trivial.
+
+  apply eq_typ_prod; trivial.
+  reflexivity.
+
+ discriminate.
+Qed.
+
+  Lemma typ_ext_abs : forall e U T M,
+    U <> kind ->
+    typ_mono e T kind ->
+    typ_equals (push_var e T) M U ->
+    typ_ext e (Abs T M) T U.
+intros.
+destruct H0; destruct H1; split.
+ apply var_ext_abs with U; trivial.
+
+ apply typ_abs; trivial.
+Qed.
+
+Lemma typ_eq_app e u v V Ur T :
+  V <> kind ->
+  Ur <> kind ->
+  sub_typ (tenv e) (subst v Ur) T ->
+  typ_equals e u (Prod V Ur) ->
+  typ_equals e v V ->
+  typ_equals e (App u v) T.
+intros Vnk Unk Tsub (uty,ueq) (vty,veq).
+split.
+ apply var_eq_app; trivial.
+
+ apply typ_subsumption with (subst v Ur); trivial.
+  apply typ_app with V; auto.
+
+  destruct Ur as [(Ur,Urm)|]; simpl; trivial.
+  discriminate.
+Qed.
+
+
+  Lemma typ_ext_app : forall e n x t u T,
+    ords e n = false ->
+    fixs e n = Some t ->
+    T <> kind ->
+    t <> kind ->
+    u <> kind ->
+    nth_error (tenv e) n = value (Prod t u) ->
+    sub_typ (tenv e) (subst x (lift_rec (S n) 1 u)) T ->
+    typ_equals e x (lift (S n) t) ->
+    typ_equals e (App (Ref n) x) T.
+intros.
+destruct H6.
+assert (typ (tenv e) (Ref n) (Prod (lift (S n) t) (lift_rec (S n) 1 u))).
+ apply typ_var0; rewrite H4; split;[discriminate|].
+ apply sub_refl.
+
+ unfold lift; rewrite eq_lift_prod.
+ reflexivity.
+split.
+ apply var_eq_rec_call with t (lift_rec (S n) 1 u); trivial.
+
+ apply typ_subsumption with (subst x (lift_rec (S n) 1 u)); auto.
+ 2:destruct u as [(u,um)|]; trivial.
+ 2:discriminate.
+ apply typ_app with (lift (S n) t); trivial.
+ destruct t as [(t,tm)|]; trivial.
+ discriminate.
+Qed.
+
+
+(** Derived rules for practical examples (basically applies subsumption beforehand) *)
+
+  Lemma typ_eq_ref' : forall e n t T,
+    spec_var e n = false ->
+    nth_error (tenv e) n = value t ->
+    t <> kind ->
+    sub_typ (tenv e) (lift (S n) t) T ->
+    typ_equals e (Ref n) T.
+intros.
+split.
+ apply var_eq_noc; apply noc_var; trivial.
+
+ apply typ_subsumption with (lift (S n) t); trivial.
+  apply typ_var; trivial.
+
+  destruct t as [(t,tm)|]; simpl in *; auto.
+  discriminate.
+Qed.
+
+(*  Lemma typ_eq_app' : forall e u v V Ur T,
+    V <> kind ->
+    Ur <> kind ->
+    sub_typ (tenv e) (subst v Ur) T ->
+    typ_equals e u (Prod V Ur) ->
+    typ_equals e v V ->
+    typ_equals e (App u v) T.
+intros.
+destruct H2.
+destruct H3.
+split.
+ apply var_eq_app; trivial.
+
+ apply typ_subsumption with (subst v Ur); trivial.
+  apply typ_app with V; auto.
+
+  destruct Ur as [(Ur,Urm)|]; simpl; trivial.
+  discriminate.
+Qed.
+*)
+(*  Lemma typ_ext_app' e n x t u T :
+    ords e n = false ->
+    fixs e n = Some t ->
+    t <> kind ->
+    u <> kind ->
+    nth_error (tenv e) n = value (Prod t u) ->
+    sub_typ (tenv e) (subst x (lift1 (S n) u)) T ->
+    typ_equals e x (lift (S n) t) ->
+    typ_equals e (App (Ref n) x) T.
+intros.
+apply typ_eq_subsumption with (2:=H4).
+ eapply typ_ext_app with (8:=H5); trivial.
+  destruct t as [(t,tm)|]; simpl; trivial; discriminate.
+
+  eapply typ_ext_ref with (4:=H3); trivial.
+
+ destruct u as [(u,um)|]; simpl; trivial; discriminate.
+Qed.
+*)
