SN_variance.v
@@ -1,0 +1,568 @@
+Require SN_ECC_Real.
+Import ZF ZFsum ZFnats ZFrelations ZFord ZFfix.
+Require Import ZFfunext ZFcoc ZFuniv_real.
+Import Sat.
+Import SN_CC_Real.SN_CC_Model SN_CC_Real.SN SN_ECC_Real.
+
+(********************************************************************************)
+(** Occurrences *)
+
+
+  (* Non-occurrence : interp do not depend on variables in set [f] *)
+  Definition noccur (f:nat->bool) (T:trm) : Prop :=
+    forall i i',
+    (forall n, if f n then True else i n == i' n) ->
+    int T i == int T i'.
+
+  Lemma noc_var : forall f n, f n = false -> noccur f (Ref n).
+red; simpl; intros.
+specialize (H0 n).
+rewrite H in H0; trivial.
+Qed.
+
+  Lemma noc_kind : forall f, noccur f kind.
+red; simpl; reflexivity.
+Qed.
+
+  Lemma noc_prop : forall f, noccur f prop.
+red; simpl; reflexivity.
+Qed.
+
+  Lemma noc_app : forall f a b,
+    noccur f a -> noccur f b -> noccur f (App a b).
+unfold noccur; simpl; intros.
+rewrite (H _ _ H1).
+rewrite (H0 _ _ H1).
+reflexivity.
+Qed.
+
+
+(********************************************************************************)
+(** Judgements with variance *)
+
+Module Beq.
+Definition t := bool.
+Definition eq := @eq bool.
+Definition eq_equiv : Equivalence eq := eq_equivalence.
+Existing Instance eq_equiv.
+End Beq.
+Module B := VarMap.Make(Beq).
+
+Module OTeq.
+Definition t := option trm.
+Definition eq := @eq (option trm).
+Definition eq_equiv : Equivalence eq := eq_equivalence.
+Existing Instance eq_equiv.
+End OTeq.
+Module OT := VarMap.Make(OTeq).
+
+(* Environments with tags on ordinal and recursive function variables *)
+Record fenv := {
+  tenv : env;
+  ords : B.map; (* variables denoting ordinals *)
+  fixs : OT.map (* variables denoting recursive functions with their domain *)
+}.
+
+Definition tinj e :=
+  Build_fenv e (B.nil false) (OT.nil None).
+
+Definition push_var e T :=
+  Build_fenv (T::tenv e) (B.cons false (ords e)) (OT.cons None (fixs e)).
+
+Definition push_fun e dom rng :=
+  Build_fenv (Prod dom rng::tenv e)
+    (B.cons false (ords e)) (OT.cons (Some dom) (fixs e)).
+
+Definition push_ord e T :=
+  Build_fenv (T::tenv e) (B.cons true (ords e)) (OT.cons None (fixs e)).
+
+
+(* Additional judgments for fix body *)
+Definition val_mono (e:fenv) i j i' j' :=
+    val_ok (tenv e) i j /\
+    val_ok (tenv e) i' j' /\
+    forall n,
+    if ords e n then i n ⊆ i' n
+    else match fixs e n with
+      Some T => forall x, x ∈ El(int T (V.shift (S n) i)) -> app (i n) x == app (i' n) x
+    | _ => i n == i' n
+    end.
+
+Lemma val_mono_refl : forall e i j,
+  val_ok (tenv e) i j -> val_mono e i j i j.
+split;[idtac|split]; simpl; auto with *.
+intro n.
+destruct (ords e n); auto with *.
+destruct (fixs e n); auto with *.
+Qed.
+
+Lemma val_push_var : forall e i j i' j' x t x' t' T,
+  val_mono e i j i' j' ->
+  x == x' ->
+  [x,t] \real int T i ->
+  [x',t'] \real int T i' ->
+  T <> kind ->
+  val_mono (push_var e T) (V.cons x i) (I.cons t j) (V.cons x' i') (I.cons t' j').
+destruct 1 as (?&?&?); split;[idtac|split]; trivial.
+ unfold push_var; simpl.
+ apply vcons_add_var; trivial.
+
+ unfold push_var; simpl.
+ apply vcons_add_var; trivial.
+
+ destruct n as [|n]; simpl; auto.
+ generalize (H1 n).
+ destruct (ords e n); trivial.
+Qed.
+
+Lemma val_push_ord : forall e i j i' j' x t x' t' T,
+  val_mono e i j i' j' ->
+  x ⊆ x' ->
+  [x,t] \real int T i ->
+  [x',t'] \real int T i' ->
+  T <> kind ->
+  val_mono (push_ord e T) (V.cons x i) (I.cons t j) (V.cons x' i') (I.cons t' j').
+destruct 1 as (?&?&?); split;[idtac|split]; trivial.
+ unfold push_ord; simpl.
+ apply vcons_add_var; trivial.
+
+ unfold push_ord; simpl.
+ apply vcons_add_var; trivial.
+
+ destruct n as [|n]; simpl; auto.
+ generalize (H1 n).
+ destruct (ords e n); trivial.
+Qed.
+
+
+Lemma val_push_fun : forall e i j i' j' f tf g tg T U,
+  val_mono e i j i' j' ->
+  [f,tf] \real int (Prod T U) i ->
+  [g,tg] \real int (Prod T U) i' ->
+  fcompat (El(int T i)) f g ->
+  val_mono (push_fun e T U) (V.cons f i) (I.cons tf j) (V.cons g i') (I.cons tg j').
+destruct 1 as (?&?&?); split;[idtac|split]; trivial.
+ unfold push_fun; simpl.
+ apply vcons_add_var; trivial.
+ discriminate.
+
+ unfold push_fun; simpl.
+ apply vcons_add_var; trivial.
+ discriminate.
+
+ destruct n as [|n]; simpl; auto.
+ generalize (H1 n).
+ destruct (ords e n); trivial.
+Qed.
+
+(** Function Extension judgment *)
+Definition fx_extends e dom M :=
+  forall i i' j j', val_mono e i j i' j' ->
+  fcompat (El(int dom i)) (int M i) (int M i').
+
+(** Covariance judgment *)
+Definition fx_sub e M :=
+  forall i i' j j', val_mono e i j i' j' ->
+  forall x t, [x,t] \real int M i -> [x,t] \real int M i'.
+
+Definition fx_subval e M :=
+  forall i i' j j', val_mono e i j i' j' -> int M i ⊆ int M i'.
+
+(** Invariance *)
+Definition fx_equals e M :=
+  forall i i' j j', val_mono e i j i' j' -> int M i == int M i'.
+
+
+Lemma El_sub e T i j i' j':
+  fx_sub e T ->
+  val_mono e i j i' j' ->
+  El (int T i) ⊆ El (int T i').
+intros.
+apply H in H0.
+red; intros.
+apply H0 with daimon.
+split;[trivial|apply varSAT].
+Qed.
+Lemma El_eq e T i j i' j':
+  fx_equals e T ->
+  val_mono e i j i' j' ->
+  El (int T i) == El (int T i').
+intros.
+apply H in H0.
+rewrite H0; reflexivity.
+Qed.
+
+Require Import Bool.
+
+Definition spec_var e n :=
+  ords e n || match fixs e n with Some _ => true | _ => false end.
+
+  Lemma fx_eq_noc : forall e t,
+    noccur (spec_var e) t ->
+    fx_equals e t.
+unfold noccur, fx_equals, spec_var; intros.
+apply H; intros.
+destruct H0 as (_,(_,H0)).
+generalize (H0 n).
+destruct (ords e n); simpl; trivial.
+destruct (fixs e n); simpl; trivial.
+Qed.
+
+  Lemma fx_eq_app : forall e u v,
+    fx_equals e u ->
+    fx_equals e v ->
+    fx_equals e (App u v).
+unfold fx_equals; intros.
+specialize H with (1:=H1).
+specialize H0 with (1:=H1).
+simpl.
+rewrite H; rewrite H0; reflexivity.
+Qed.
+
+  Lemma fx_eq_abs : forall e T M,
+    T <> kind ->
+    fx_equals e T ->
+    fx_equals (push_var e T) M ->
+    fx_equals e (Abs T M).
+unfold fx_equals; intros.
+simpl.
+apply lam_ext; eauto.
+red; intros.
+apply H1 with (I.cons daimon j) (I.cons daimon j').
+specialize H0 with (1:=H2).
+apply val_push_var; auto.
+ split; trivial.
+ apply varSAT.
+
+ split.
+ 2:apply varSAT.
+ unfold inX; rewrite <- H4; rewrite <- H0; trivial.
+Qed.
+
+  Lemma fx_eq_rec_call : forall e n x T U,
+    ords e n = false ->
+    fixs e n = Some T ->
+    T <> kind ->
+    typ (tenv e) (Ref n) (Prod (lift (S n) T) U) ->
+    fx_equals e x ->
+    typ (tenv e) x (lift (S n) T) ->
+    fx_equals e (App (Ref n) x).
+unfold fx_equals; intros.
+simpl.
+specialize H3 with (1:=H5).
+rewrite <- H3.
+destruct H5 as (Hty,(Hty',Hrec)).
+specialize Hrec with n.
+rewrite H in Hrec; rewrite H0 in Hrec.
+apply Hrec.
+red in H4; specialize H4 with (1:=Hty); trivial.
+apply in_int_not_kind in H4; trivial.
+2:destruct T;[discriminate|elim H1;reflexivity].
+destruct H4 as (?,_ ).
+unfold inX in H4.
+unfold lift in H4; rewrite int_lift_rec_eq in H4.
+rewrite V.lams0 in H4; trivial.
+Qed.
+
+  (* Covariance *)
+
+  Lemma fx_equals_subval : forall e M, fx_equals e M -> fx_subval e M.
+unfold fx_subval, fx_equals; intros.
+apply H in H0.
+rewrite <- H0; reflexivity.
+Qed.
+
+  Lemma fx_equals_sub : forall e M, fx_equals e M -> fx_sub e M.
+unfold fx_sub, fx_equals; intros.
+apply H in H0.
+destruct H1.
+split.
+ red.
+ rewrite <- H0; trivial.
+
+ rewrite <- H0; trivial.
+Qed.
+
+  Lemma var_sub : forall e n,
+    ords e n = true ->
+    fx_subval e (Ref n).
+unfold fx_subval; intros.
+destruct H0 as (_,(_,H0)).
+generalize (H0 n); rewrite H.
+simpl; trivial.
+Qed.
+
+Lemma fx_sub_prod : forall e T U,
+  T <> kind ->
+  fx_equals e T ->
+  fx_sub (push_var e T) U ->
+  fx_sub e (Prod T U).
+red; intros.
+red in H0; specialize H0 with (1:=H2).
+destruct H3.
+red in H3.
+rewrite El_int_prod in H3.
+rewrite Real_int_prod in H4; trivial.
+apply and_split; intros.
+ red; rewrite El_int_prod.
+ revert H3; apply cc_prod_covariant; intros.
+  do 2 red; intros.
+  rewrite H5; reflexivity.
+
+  rewrite H0; reflexivity.
+
+  apply El_sub with (1:=H1) (j:=I.cons daimon j) (j':=I.cons daimon j').
+  apply val_push_var; auto with *.
+   split;[trivial|apply varSAT].
+   split;[|apply varSAT].
+   red; rewrite <- H0; trivial.
+
+ red in H5; rewrite El_int_prod in H5.
+ rewrite Real_int_prod; trivial.
+ apply interSAT_intro' with
+   (F:=fun v => prodSAT(Real(int T i') v)(Real(int U (V.cons v i'))(cc_app x v))).
+  apply sat_sn in H4; trivial.
+ intros.
+ rewrite <- H0 in H6.
+ specialize interSAT_elim with (1:=H4) (x:=exist (fun x=> x ∈ El(int T i)) x0 H6); simpl proj1_sig; intros.
+ revert H7; apply prodSAT_mono.
+  do 2 red; intros.
+  rewrite <- H0 in H7; trivial.
+
+  red; intros.
+  apply H1 with (i:=V.cons x0 i) (j:=I.cons daimon j) (j':=I.cons daimon j').
+   apply val_push_var; auto with *.
+   split; trivial; apply varSAT.
+   split.
+    red; rewrite <- H0; trivial.
+    apply varSAT.
+
+   split; trivial.
+   unfold inX; apply cc_prod_elim with (1:=H3); trivial.
+Qed.
+
+  (* Function subtyping *)
+
+  Lemma fx_abs : forall e U T M,
+    T <> kind ->
+    fx_sub e T ->
+    fx_equals (push_var e T) M ->
+    typ (T::tenv e) M U ->
+    U <> kind ->
+    fx_extends e T (Abs T M).
+unfold fx_equals, fx_extends; intros.
+specialize El_sub with (1:=H0)(2:=H4); clear H0; intro H0.
+simpl.
+red; intros.
+rewrite beta_eq; try assumption.
+ assert (H5' := H0 _ H5).
+ rewrite beta_eq; trivial.
+  apply H1 with (I.cons daimon j) (I.cons daimon j').
+  apply val_push_var; auto with *.
+   split; [trivial|apply varSAT].
+
+   split; [trivial|apply varSAT].
+
+  red; red; intros.
+  rewrite H7; reflexivity.
+
+ red; red; intros.
+ rewrite H7; reflexivity.
+Qed.
+
+(****************************************************************************************)
+(** Compound judgements : typing + variance *)
+
+Definition typ_ext e M A B :=
+  fx_extends e A M /\ typ (tenv e) M (Prod A B).
+
+Definition typ_mono e M :=
+  fx_sub e M /\ typs (tenv e) M.
+
+Definition typ_monoval e M T :=
+  fx_subval e M /\ typ (tenv e) M T.
+
+Definition typ_impl e M T :=
+  fx_equals e M /\ typ (tenv e) M T.
+
+Instance typ_impl_morph e : Proper (eq_trm ==> eq_trm ==> iff) (typ_impl e).
+apply morph_impl_iff2; auto with *.
+do 4 red; intros.
+destruct H1; split.
+ red; intros.
+ rewrite <- H; eauto.
+
+ rewrite <- H; rewrite <- H0; eauto.
+Qed.
+
+Lemma typ_var_impl : forall e n t T,
+    spec_var e n = false ->
+    nth_error (tenv e) n = value t ->
+    t <> kind ->
+    T <> kind ->
+    sub_typ (tenv e) (lift (S n) t) T ->
+    typ_impl e (Ref n) T.
+intros.
+split.
+ apply fx_eq_noc; apply noc_var; trivial.
+
+ apply typ_subsumption with (lift (S n) t); trivial.
+  apply typ_var; trivial.
+
+  destruct t as [(t,tm)|]; simpl in *; auto.
+  discriminate.
+Qed.
+
+  Lemma impl_abs : forall e s1 U T T' M,
+    T <> kind ->
+    U <> kind ->
+    s1=prop \/ s1=kind ->
+    eq_typ (tenv e) T T' ->
+    typ_impl e T s1 ->
+    typ_impl (push_var e T) M U ->
+    typ_impl e (Abs T M) (Prod T' U).
+intros.
+destruct H3; destruct H4.
+split.
+ apply fx_eq_abs; trivial.
+
+ apply typ_conv with (Prod T U); auto.
+  apply typ_abs; trivial.
+  destruct H1; subst s1; red; auto.
+
+  apply eq_typ_prod; trivial.
+  reflexivity.
+
+  discriminate.
+
+  discriminate.
+Qed.
+
+Lemma impl_app : forall e u v V Ur T,
+  T <> kind ->
+  V <> kind ->
+  Ur <> kind ->
+  sub_typ (tenv e) (subst v Ur) T ->
+  typ_impl e u (Prod V Ur) ->
+  typ_impl e v V ->
+  typ_impl e (App u v) T.
+intros.
+destruct H3.
+destruct H4.
+split.
+ apply fx_eq_app; trivial.
+
+ apply typ_subsumption with (subst v Ur); trivial.
+  apply typ_app with V; auto.
+
+  destruct Ur as [(Ur,Urm)|]; simpl; trivial.
+  discriminate.
+Qed.
+
+
+  Lemma typ_var_mono : forall e n t T,
+    ords e n = true ->
+    nth_error (tenv e) n = value t ->
+    T <> kind ->
+    t <> kind ->
+    sub_typ (tenv e) (lift (S n) t) T ->
+    typ_monoval e (Ref n) T.
+intros.
+split.
+ apply var_sub; trivial.
+
+ apply typ_subsumption with (lift (S n) t); trivial.
+  apply typ_var; trivial.
+
+  destruct t as [(t,tm)|]; simpl in *; auto.
+  discriminate.
+Qed.
+
+  Lemma ext_abs : forall e U T M,
+    T <> kind ->
+    U <> kind ->
+    typ_mono e T ->
+    typ_impl (push_var e T) M U ->
+    typ_ext e (Abs T M) T U.
+intros.
+destruct H1; destruct H2; split.
+ apply fx_abs with U; trivial.
+
+ apply typ_abs; trivial.
+Qed.
+
+(*************)
+
+  Lemma impl_call : forall e n x t u T,
+    ords e n = false ->
+    fixs e n = Some t ->
+    T <> kind ->
+    t <> kind ->
+    u <> kind ->
+    nth_error (tenv e) n = value (Prod t u) ->
+    sub_typ (tenv e) (subst x (lift_rec (S n) 1 u)) T ->
+    typ_impl e x (lift (S n) t) ->
+    typ_impl e (App (Ref n) x) T.
+intros.
+destruct H6.
+assert (typ (tenv e) (Ref n) (Prod (lift (S n) t) (lift_rec (S n) 1 u))).
+ apply typ_var0; rewrite H4; split;[discriminate|].
+ apply sub_refl.
+
+ unfold lift; rewrite red_lift_prod.
+ reflexivity.
+split.
+ apply fx_eq_rec_call with t (lift_rec (S n) 1 u); trivial.
+
+ apply typ_subsumption with (subst x (lift_rec (S n) 1 u)); auto.
+ 2:destruct u as [(u,um)|]; trivial.
+ 2:discriminate.
+ apply typ_app with (lift (S n) t); trivial.
+ destruct t as [(t,tm)|]; trivial.
+ discriminate.
+ destruct u as [(u,um)|]; trivial.
+ discriminate.
+Qed.
+
+
+(** Variance and ordinals *)
+Require Import SN_ord.
+
+  Lemma OSucc_sub : forall e O,
+    fx_subval e O ->
+    fx_subval e (OSucc O).
+unfold fx_subval; simpl; intros.
+unfold osucc.
+red; intros.
+rewrite subset_ax in H1 |-*.
+destruct H1; split; auto.
+revert H1; apply power_mono.
+eauto.
+Qed.
+
+  Lemma OSucc_fx_sub : forall e O o,
+    isOrd o ->
+    zero ∈ o ->
+    typ_monoval e O (Ordt o)->
+    typ_monoval e (OSucc O) (Ordt (osucc o)).
+destruct 3.
+split.
+ apply OSucc_sub; trivial.
+
+ red; simpl; intros.
+ apply in_int_intro; try discriminate.
+ destruct tyord_inv with (3:=H2)(4:=H3) as (_,(?,_)); trivial.
+ assert (osucc (int O i) ∈ El (int (Ordt (osucc o)) i)).
+  rewrite El_int_ord.
+  apply lt_osucc_compat; trivial.
+  apply ole_lts; auto.
+ split; simpl; trivial.
+ rewrite Real_def; auto with *.
+  assert (h:= H2 _ _ H3).
+  apply in_int_sn in h.
+  simpl; trivial.
+
+  simpl.
+  apply cc_bot_intro.
+  apply lt_osucc_compat; trivial.
+Qed.
